BoogieLang/Ast_Cfg_Transformation.thy
@@ -1,0 +1,1402 @@
+theory Ast_Cfg_Transformation 
+   imports Main
+          "Boogie_Lang.Ast"
+          "Boogie_Lang.Semantics"
+          "Boogie_Lang.BackedgeElim"
+begin 
+
+text \<open>The following are various miscellaneous helper lemmas used later in the proofs of the local and global relation lemmas.\<close>
+
+lemmas converse_rtranclp_induct3 =
+  converse_rtranclp_induct [of _ "(ax, ay, az)" "(bx, by, bz)", split_rule, consumes 1, case_names refl step]
+
+lemmas converse_rtranclpE3 = converse_rtranclpE [of _ "(xa,xb,xc)" "(za,zb,zc)", split_rule]
+
+lemma final_is_static: 
+  assumes "is_final ((BigBlock name [] None None), start_cont, start_state)"
+  shows "\<And>A M \<Lambda> \<Gamma> \<Omega> T end_bb end_cont end_state. 
+         (red_bigblock A M \<Lambda> \<Gamma> \<Omega> T ((BigBlock name [] None None), start_cont, start_state) (end_bb, end_cont, end_state)) \<Longrightarrow> 
+         ((end_bb, end_cont, end_state) = ((BigBlock name [] None None), start_cont, start_state))" 
+  using assms 
+proof -
+  fix A M \<Lambda> \<Gamma> \<Omega> T end_bb  end_cont end_state
+  have cont_eq: "start_cont = KStop" using assms is_final.elims(1) by blast  
+
+  assume prem1: "(red_bigblock A M \<Lambda> \<Gamma> \<Omega> T ((BigBlock name [] None None), start_cont, start_state) (end_bb, end_cont, end_state))"
+  from prem1 show "((end_bb, end_cont, end_state) = ((BigBlock name [] None None), start_cont, start_state))" using cont_eq
+  proof cases 
+    case RedFailure_or_Magic thus ?thesis using cont_eq by blast
+  qed auto
+qed
+
+lemma final_is_static_propagate:
+  assumes "rtranclp (red_bigblock A M \<Lambda> \<Gamma> \<Omega> T) start_config  end_config" 
+  and "is_final start_config"
+  and "start_config = ((BigBlock name [] None None), start_cont, start_state)"
+  shows "end_config = ((BigBlock name [] None None), start_cont, start_state)"
+  using assms
+proof (induction rule: rtranclp.induct)
+  case (rtrancl_refl a)
+  then show ?case using assms by simp
+next
+  case (rtrancl_into_rtrancl a b c)
+  then have inter_is_same: "b = (BigBlock name [] None None, start_cont, start_state)" and inter_is_final: "is_final b" by auto
+  have "start_cont = KStop" using rtrancl_into_rtrancl(4) is_final.elims(1) rtrancl_into_rtrancl.prems(2) by blast
+
+  from rtrancl_into_rtrancl(2) show ?case
+    using inter_is_same inter_is_final \<open>start_cont = KStop\<close>
+  proof cases
+    case RedFailure_or_Magic thus ?thesis using inter_is_same inter_is_final \<open>start_cont = KStop\<close> by (auto simp add: RedFailure_or_Magic)
+  qed auto
+qed
+
+
+lemma magic_propagates: 
+  assumes "A,M,\<Lambda>,\<Gamma>,\<Omega>,T \<turnstile> (bb, cont, Magic) -n\<longrightarrow>^j (reached_bb, reached_cont, reached_state)"
+    shows "reached_state = Magic"
+  using assms
+proof (cases j)
+  case 0 
+  hence "(reached_bb, reached_cont, reached_state) = (bb, cont, Magic)" using assms by fastforce
+  thus ?thesis by simp
+next
+  case (Suc j')
+  from this obtain first_inter where 
+    red1: "A,M,\<Lambda>,\<Gamma>,\<Omega>,T \<turnstile> \<langle>(bb, cont, Magic)\<rangle> \<longrightarrow> first_inter" and red_rest: "A,M,\<Lambda>,\<Gamma>,\<Omega>,T \<turnstile> first_inter -n\<longrightarrow>^j' (reached_bb, reached_cont, reached_state)"
+    by (metis assms relpowp_Suc_E2)
+  hence reached_conj: "((get_state first_inter) = Magic) \<and> ((is_final first_inter) = True)" 
+  proof cases
+    case RedFailure_or_Magic thus ?thesis by simp
+  qed
+  hence magic_reached: "(get_state first_inter) = Magic" by simp
+  have final_config: "is_final first_inter" using reached_conj by simp
+  hence "\<exists> name. first_inter = ((BigBlock name [] None None), KStop, Magic)" using magic_reached
+    by (metis get_state.simps is_final.elims(2))
+  from this obtain name1 where concrete: "first_inter = ((BigBlock name1 [] None None), KStop, Magic)" 
+    by blast 
+
+  from red_rest show ?thesis using final_config magic_reached concrete final_is_static_propagate by (metis prod.inject relpowp_imp_rtranclp)
+qed 
+
+
+lemma strictly_smaller_helper2: "j'' < j' \<Longrightarrow> j = Suc j' \<Longrightarrow> j'' < j"
+  by simp
+
+lemma steps_trans_helper:
+  assumes "A,M,\<Lambda>,\<Gamma>,\<Omega>,T \<turnstile>(bb0, cont0, Normal ns1'') -n\<longrightarrow>^j' (reached_bb, reached_cont, reached_state)"
+  shows "rtranclp (red_bigblock A M \<Lambda> \<Gamma> \<Omega> T) (bb0, cont0, Normal ns1'') (reached_bb, reached_cont, reached_state)"
+  using assms
+proof -
+  from assms(1) show ?thesis by (simp add: relpowp_imp_rtranclp)
+qed
+
+lemma endblock_skip:
+  assumes "A,M,\<Lambda>,\<Gamma>,\<Omega>,T \<turnstile>(BigBlock None [] None None, KEndBlock (KSeq bb_next cont0), Normal ns3) -n\<longrightarrow>^l (reached_bb, reached_cont, reached_state)"
+  shows "(valid_configuration A \<Lambda> \<Gamma> \<Omega> [] reached_bb reached_cont reached_state) \<or> 
+            (\<exists> l2. (A,M,\<Lambda>,\<Gamma>,\<Omega>,T \<turnstile>(bb_next, cont0, Normal ns3) -n\<longrightarrow>^l2 (reached_bb, reached_cont, reached_state)) \<and> (l = Suc (Suc l2)) )"
+  using assms
+proof (cases l)
+  case 0
+  then show ?thesis by (metis Ast.valid_configuration_def assms get_state.simps is_final.simps(6) relpowp_fun_conv state.simps(3))
+next
+  case 1: (Suc l1)
+  then show ?thesis 
+  proof (cases l1)
+    case 0
+    from 1 assms this have "(red_bigblock A M \<Lambda> \<Gamma> \<Omega> T (BigBlock None [] None None, KEndBlock (KSeq bb_next cont0), Normal ns3) (reached_bb, reached_cont, reached_state))"
+      by fastforce
+    then show ?thesis
+    proof cases
+      case RedSkipEndBlock thus ?thesis by (simp add: Ast.valid_configuration_def)
+    qed auto
+  next
+    case 2: (Suc l2)
+    from 2 1 have "l = Suc (Suc l2)" by auto
+    from 2 1 assms obtain inter_bb inter_cont inter_state inter_bb2 inter_cont2 inter_state2 where
+      step1: "(red_bigblock A M \<Lambda> \<Gamma> \<Omega> T (BigBlock None [] None None, KEndBlock (KSeq bb_next cont0), Normal ns3) (inter_bb, inter_cont, inter_state))" and 
+      step2: "(red_bigblock A M \<Lambda> \<Gamma> \<Omega> T (inter_bb, inter_cont, inter_state) (inter_bb2, inter_cont2, inter_state2))" and
+      rest: "A,M,\<Lambda>,\<Gamma>,\<Omega>,T \<turnstile>(inter_bb2, inter_cont2, inter_state2) -n\<longrightarrow>^l2 (reached_bb, reached_cont, reached_state)" 
+      by (metis (no_types, opaque_lifting) prod_cases3 relpowp_Suc_D2)
+    from this step1 have "(inter_bb, inter_cont, inter_state) = (BigBlock None [] None None, (KSeq bb_next cont0), Normal ns3)"
+    proof cases
+      case RedSkipEndBlock thus ?thesis 
+        by blast
+    qed auto
+    from step2 this have "(inter_bb2, inter_cont2, inter_state2) = (bb_next, cont0, Normal ns3)" 
+    proof cases 
+      case RedSkip thus ?thesis  using \<open>(inter_bb, inter_cont, inter_state) = (BigBlock None [] None None, KSeq bb_next cont0, Normal ns3)\<close> by fastforce
+    qed auto
+    hence "(A,M,\<Lambda>,\<Gamma>,\<Omega>,T \<turnstile>(bb_next, cont0, Normal ns3) -n\<longrightarrow>^l2 (reached_bb, reached_cont, reached_state)) \<and> (l = Suc (Suc l2))" using rest \<open>l = Suc (Suc l2)\<close> by simp
+    then show ?thesis by blast
+  qed
+qed
+
+lemma endblock_skip_wrapper:
+  assumes "A,M,\<Lambda>,\<Gamma>,\<Omega>,T \<turnstile>(BigBlock None [] None None, KEndBlock (KSeq (BigBlock name [] (Some (WhileWrapper str)) tr) cont0), Normal ns3) -n\<longrightarrow>^l (reached_bb, reached_cont, reached_state)"
+  shows "(valid_configuration A \<Lambda> \<Gamma> \<Omega> [] reached_bb reached_cont reached_state) \<or> 
+         (\<exists> l3. (A,M,\<Lambda>,\<Gamma>,\<Omega>,T \<turnstile>((BigBlock name [] (Some str) tr), KEndBlock cont0, Normal ns3) -n\<longrightarrow>^l3 (reached_bb, reached_cont, reached_state)) \<and> (l = Suc (Suc (Suc l3))) )"
+  using assms
+proof (cases l)
+  case 0
+  then show ?thesis by (metis Ast.valid_configuration_def assms get_state.simps is_final.simps(6) relpowp_fun_conv state.simps(3))
+next
+  case 1: (Suc l1)
+  then show ?thesis 
+    proof (cases l1)
+      case 0
+      from 1 assms this have 
+        "(red_bigblock A M \<Lambda> \<Gamma> \<Omega> T (BigBlock None [] None None, KEndBlock (KSeq (BigBlock name [] (Some (WhileWrapper str)) tr) cont0), Normal ns3) (reached_bb, reached_cont, reached_state))"
+        by fastforce
+      then show ?thesis
+      proof cases
+        case RedSkipEndBlock thus ?thesis by (simp add: Ast.valid_configuration_def)
+      qed auto
+    next
+      case 2: (Suc l2)
+      then show ?thesis
+      proof (cases l2)
+        case 0 
+        from 2 1 have "l = Suc (Suc l2)" by auto
+        from 2 1 assms obtain inter_bb inter_cont inter_state  where
+          step1: "(red_bigblock A M \<Lambda> \<Gamma> \<Omega> T (BigBlock None [] None None, KEndBlock (KSeq (BigBlock name [] (Some (WhileWrapper str)) tr) cont0), Normal ns3) (inter_bb, inter_cont, inter_state))" and 
+          step2: "(red_bigblock A M \<Lambda> \<Gamma> \<Omega> T (inter_bb, inter_cont, inter_state) (reached_bb, reached_cont, reached_state))" 
+          using "0" by auto
+        from this step1 have "(inter_bb, inter_cont, inter_state) = (BigBlock None [] None None, (KSeq (BigBlock name [] (Some (WhileWrapper str)) tr) cont0), Normal ns3)"
+        proof cases
+          case RedSkipEndBlock thus ?thesis 
+            by blast
+        qed auto
+        from step2 this have "(reached_bb, reached_cont, reached_state) = ((BigBlock name [] (Some (WhileWrapper str)) tr), cont0, Normal ns3)" 
+        proof cases 
+          case RedSkip thus ?thesis  using \<open>(inter_bb, inter_cont, inter_state) = (BigBlock None [] None None, (KSeq (BigBlock name [] (Some (WhileWrapper str)) tr) cont0), Normal ns3)\<close> by fastforce
+        qed auto
+        then show ?thesis by (simp add: Ast.valid_configuration_def)
+      next
+        case 3: (Suc l3)
+        from 3 2 1 have "l = Suc (Suc (Suc l3))" by auto
+        from 3 2 1 assms obtain inter_bb inter_cont inter_state inter_bb2 inter_cont2 inter_state2 inter_bb3 inter_cont3 inter_state3 where
+          step1: "(red_bigblock A M \<Lambda> \<Gamma> \<Omega> T (BigBlock None [] None None, KEndBlock (KSeq (BigBlock name [] (Some (WhileWrapper str)) tr) cont0), Normal ns3) (inter_bb, inter_cont, inter_state))" and 
+          step2: "(red_bigblock A M \<Lambda> \<Gamma> \<Omega> T (inter_bb, inter_cont, inter_state) (inter_bb2, inter_cont2, inter_state2))" and 
+          step3: "(red_bigblock A M \<Lambda> \<Gamma> \<Omega> T (inter_bb2, inter_cont2, inter_state2) (inter_bb3, inter_cont3, inter_state3))" and
+          rest: "A,M,\<Lambda>,\<Gamma>,\<Omega>,T \<turnstile> (inter_bb3, inter_cont3, inter_state3) -n\<longrightarrow>^l3 (reached_bb, reached_cont, reached_state)" 
+          by (metis (no_types, opaque_lifting) get_state.cases relpowp_Suc_D2)
+  
+        from this step1 have "(inter_bb, inter_cont, inter_state) = (BigBlock None [] None None, (KSeq (BigBlock name [] (Some (WhileWrapper str)) tr) cont0), Normal ns3)"
+        proof cases
+          case RedSkipEndBlock thus ?thesis 
+            by blast
+        qed auto
+        from step2 this have "(inter_bb2, inter_cont2, inter_state2) = ((BigBlock name [] (Some (WhileWrapper str)) tr), cont0, Normal ns3)" 
+        proof cases 
+          case RedSkip thus ?thesis  using \<open>(inter_bb, inter_cont, inter_state) = (BigBlock None [] None None, (KSeq (BigBlock name [] (Some (WhileWrapper str)) tr) cont0), Normal ns3)\<close> by fastforce
+        qed auto
+        from step3 this have "(inter_bb3, inter_cont3, inter_state3) = ((BigBlock name [] (Some str) tr), KEndBlock cont0, Normal ns3)"
+        proof cases
+          case RedParsedWhileWrapper thus ?thesis using \<open>(inter_bb2, inter_cont2, inter_state2) = (BigBlock name [] (Some (WhileWrapper str)) tr, cont0, Normal ns3)\<close> by fastforce 
+        qed auto
+        hence "(A,M,\<Lambda>,\<Gamma>,\<Omega>,T \<turnstile>((BigBlock name [] (Some str) tr), KEndBlock cont0, Normal ns3) -n\<longrightarrow>^l3 (reached_bb, reached_cont, reached_state)) \<and> (l = Suc (Suc (Suc l3)))" 
+          using \<open>l = Suc (Suc (Suc l3))\<close> rest by blast
+        thus ?thesis by blast
+    qed
+  qed
+qed
+
+text \<open>Local lemmas: The following are lemmas proving local relations between various kinds of ast-bigblocks and cfg-blocks\<close>
+
+text \<open>Local relation between an ast-bigblock starting with a non-empty set of simple commands and a cfg-block containing the same simple commands\<close>
+lemma block_local_rel_generic:
+  assumes block_rel: "ast_cfg_rel guard invs (BigBlock name cs1 any_str any_tr) cs2"
+  and "cs1 \<noteq> Nil"
+  and "cs2 \<noteq> Nil"
+  and "guard = None"
+  and "invs = []"
+  and Red_bb_to: "red_bigblock A M \<Lambda> \<Gamma> \<Omega> T ((BigBlock name cs1 any_str any_tr), cont0, (Normal ns1)) (reached_bb, reached_cont, reached_state)" 
+  and Red_impl: "(\<And> s2'.((red_cmd_list A M \<Lambda> \<Gamma> \<Omega> cs2 (Normal ns1) s2') \<Longrightarrow> (s2' \<noteq> Failure)))" 
+  shows "reached_state \<noteq> Failure  \<and>
+         (\<forall>ns1'. reached_state = Normal ns1' \<longrightarrow> (A,M,\<Lambda>,\<Gamma>,\<Omega> \<turnstile> \<langle>cs2, Normal ns1\<rangle> [\<rightarrow>] Normal ns1'))" 
+  using assms
+proof (induction arbitrary: ns1)
+  case (Rel_Main_test name cs1 any_str any_tr)
+  thus ?case
+  proof (cases cs1)
+    case Nil
+    then show ?thesis using Rel_Main_test(2) by simp
+  next
+    case (Cons a list)
+    then have "red_bigblock A M \<Lambda> \<Gamma> \<Omega> T ((BigBlock name (a#list) any_str any_tr), cont0, (Normal ns1)) (reached_bb, reached_cont, reached_state)" 
+      using Rel_Main_test(5) by simp
+    then have "A,M,\<Lambda>,\<Gamma>,\<Omega> \<turnstile> \<langle>(a#list), Normal ns1\<rangle> [\<rightarrow>] reached_state" using Rel_Main_test(5) 
+    proof cases
+      case RedSimpleCmds thus ?thesis by (simp add: RedSimpleCmds)
+    qed
+    then have "A,M,\<Lambda>,\<Gamma>,\<Omega> \<turnstile> \<langle>cs1, Normal ns1\<rangle> [\<rightarrow>] reached_state" using Cons by simp
+    
+    then show ?thesis using Rel_Main_test(6) by auto
+  qed 
+qed auto
+
+text \<open>Local relation between (an ast-bigblock starting with a non-empty set of simple commands 
+               and (is the first ast-bigblock in the then-branch of an if-statement or is the first ast-bigblock in the body of a while-loop)) 
+       and a cfg-block containing the same simple commands\<close>
+lemma block_local_rel_guard_true:
+  assumes block_rel: "ast_cfg_rel None [] (BigBlock name cs1 any_str any_tr) cs2"
+  and "cs1 \<noteq> Nil"
+  and "cs2 \<noteq> Nil"
+  and "c = Assume block_guard"
+  and trace_is_possible: "A,\<Lambda>,\<Gamma>,\<Omega> \<turnstile> \<langle>block_guard, ns1\<rangle> \<Down> LitV (LBool True)"
+  and Red_bb_to: "red_bigblock A M \<Lambda> \<Gamma> \<Omega> T ((BigBlock name cs1 any_str any_tr), cont0, (Normal ns1)) (reached_bb, reached_cont, reached_state)" 
+  and Red_impl: "(\<And> s2'.((red_cmd_list A M \<Lambda> \<Gamma> \<Omega> (c#cs2) (Normal ns1) s2') \<Longrightarrow> (s2' \<noteq> Failure)))" 
+  shows "reached_state \<noteq> Failure  \<and>
+         (\<forall>ns1'. reached_state = Normal ns1' \<longrightarrow> (A,M,\<Lambda>,\<Gamma>,\<Omega> \<turnstile> \<langle>(c#cs2), Normal ns1\<rangle> [\<rightarrow>] Normal ns1'))" 
+  using assms 
+proof cases
+  case Rel_Main_test
+  have Red_impl_extended: "(\<And> s2'.((red_cmd_list A M \<Lambda> \<Gamma> \<Omega> cs2 (Normal ns1) s2') \<Longrightarrow> (s2' \<noteq> Failure)))" 
+    using trace_is_possible \<open>c = Assume block_guard\<close> Red_impl RedAssumeOk RedCmdListCons by blast
+  hence snd_step_to_end: "reached_state \<noteq> Failure  \<and> (\<forall>ns1'. reached_state = Normal ns1' \<longrightarrow> (A,M,\<Lambda>,\<Gamma>,\<Omega> \<turnstile> \<langle>cs2, Normal ns1\<rangle> [\<rightarrow>] Normal ns1'))"
+    using Red_bb_to assms(2-3) block_local_rel_generic block_rel 
+    by blast 
+  have push_one_cmd: "A,M,\<Lambda>,\<Gamma>,\<Omega> \<turnstile> \<langle>c, Normal ns1\<rangle> \<rightarrow> Normal ns1" 
+    using \<open>c = Assume block_guard\<close> trace_is_possible 
+    by (simp only: RedAssumeOk)
+  then show ?thesis using snd_step_to_end  by (simp add: RedCmdListCons)
+qed auto
+
+text \<open>Local relation between (an ast-bigblock starting with a non-empty set of simple commands 
+               and (is the first ast-bigblock in the else-branch of an if-statement or is the first ast-bigblock after a while-loop)) 
+       and a cfg-block containing the same simple commands\<close>
+lemma block_local_rel_guard_false:
+  assumes block_rel: "ast_cfg_rel None [] (BigBlock name cs1 any_str any_tr) cs2"
+  and "cs1 \<noteq> Nil"
+  and "cs2 \<noteq> Nil"
+  and "(UnOp Not block_guard) \<sim> b "
+  and "c = Assume b"
+  and trace_is_possible: "A,\<Lambda>,\<Gamma>,\<Omega> \<turnstile> \<langle>(UnOp Not block_guard), ns1\<rangle> \<Down> LitV (LBool True)"
+  and Red_bb_to: "red_bigblock A M \<Lambda> \<Gamma> \<Omega> T ((BigBlock name cs1 any_str any_tr), cont0, (Normal ns1)) (reached_bb, reached_cont, reached_state)" 
+  and Red_impl: "(\<And> s2'.((red_cmd_list A M \<Lambda> \<Gamma> \<Omega> (c#cs2) (Normal ns1) s2') \<Longrightarrow> (s2' \<noteq> Failure)))" 
+  shows "reached_state \<noteq> Failure  \<and>
+         (\<forall>ns1'. reached_state = Normal ns1' \<longrightarrow> (A,M,\<Lambda>,\<Gamma>,\<Omega> \<turnstile> \<langle>(c#cs2), Normal ns1\<rangle> [\<rightarrow>] Normal ns1'))" 
+  using assms 
+proof cases
+  case Rel_Main_test
+  have Red_impl_extended: "(\<And> s2'.((red_cmd_list A M \<Lambda> \<Gamma> \<Omega> cs2 (Normal ns1) s2') \<Longrightarrow> (s2' \<noteq> Failure)))" 
+    using trace_is_possible \<open>c = Assume b\<close> \<open>(UnOp Not block_guard) \<sim> b\<close> equiv_preserves_value  Red_impl RedAssumeOk RedCmdListCons by metis
+  hence snd_step_to_end: "reached_state \<noteq> Failure  \<and> (\<forall>ns1'. reached_state = Normal ns1' \<longrightarrow> (A,M,\<Lambda>,\<Gamma>,\<Omega> \<turnstile> \<langle>cs2, Normal ns1\<rangle> [\<rightarrow>] Normal ns1'))"
+    using Red_bb_to assms(2-3) block_local_rel_generic block_rel 
+    by blast 
+  have equiv: "A,\<Lambda>,\<Gamma>,\<Omega> \<turnstile> \<langle>b, ns1\<rangle> \<Down> BoolV True" 
+    using trace_is_possible equiv_preserves_value \<open>(UnOp Not block_guard) \<sim> b\<close>
+    by metis
+  hence push_one_cmd: "A,M,\<Lambda>,\<Gamma>,\<Omega> \<turnstile> \<langle>c, Normal ns1\<rangle> \<rightarrow> Normal ns1" 
+    using \<open>c = Assume b\<close> trace_is_possible equiv_preserves_value
+    by (auto simp add: RedAssumeOk)
+  then show ?thesis using snd_step_to_end  by (simp add: RedCmdListCons)
+qed auto
+
+text \<open>Local relation between a loop-only(no simple commands) ast-bigblock and a corresponding cfg-block containing assertions of the loop invariants\<close>
+lemma block_local_rel_loop_head:
+  assumes block_rel: "ast_cfg_rel None assert_invs (BigBlock name [] (Some (ParsedWhile loop_guard invs (bb0#body_bbs))) any_tr) assertions"
+  and "assert_invs = map inv_into_assertion invs"
+  and Red_bb: "red_bigblock A M \<Lambda> \<Gamma> \<Omega> T ((BigBlock name [] (Some (ParsedWhile loop_guard invs (bb0#body_bbs))) any_tr), cont0, (Normal ns1)) (reached_bb, reached_cont, reached_state)" 
+  and Red_impl: "(\<And> s2'.((red_cmd_list A M \<Lambda> \<Gamma> \<Omega> assertions (Normal ns1) s2') \<Longrightarrow> (s2' \<noteq> Failure)))"
+  shows "reached_state \<noteq> Failure  \<and>
+         (\<forall>ns1'. reached_state = Normal ns1' \<longrightarrow> (A,M,\<Lambda>,\<Gamma>,\<Omega> \<turnstile> \<langle>assertions, Normal ns1\<rangle> [\<rightarrow>] Normal ns1'))" 
+  using assms
+proof cases
+  case Rel_Invs
+  hence "assertions = map inv_into_assertion invs" using assms(2) by simp
+  from Red_bb show ?thesis
+  proof cases
+    case RedParsedWhileTrue thus ?thesis using \<open>assertions = (map inv_into_assertion invs)\<close>  by (simp add: asserts_hold_if_invs_hold)
+  next
+    case RedParsedWhileFalse thus ?thesis using \<open>assertions = (map inv_into_assertion invs)\<close>  by (simp add: asserts_hold_if_invs_hold)
+  next
+    case RedParsedWhile_InvFail thus ?thesis using Red_impl \<open>assertions = map inv_into_assertion invs\<close> one_inv_fails_assertions by blast
+  qed auto
+next
+  case Rel_Main_test
+  hence "assertions = map inv_into_assertion invs" using assms(2) by simp
+  from Red_bb show ?thesis
+  proof cases
+    case RedParsedWhileTrue thus ?thesis using \<open>assertions = (map inv_into_assertion invs)\<close>  by (simp add: asserts_hold_if_invs_hold)
+  next
+    case RedParsedWhileFalse thus ?thesis using \<open>assertions = (map inv_into_assertion invs)\<close>  by (simp add: asserts_hold_if_invs_hold)
+  next
+    case RedParsedWhile_InvFail thus ?thesis using Red_impl \<open>assertions = map inv_into_assertion invs\<close> one_inv_fails_assertions by blast
+  qed auto
+qed
+
+text \<open>Global lemmas: The following are lemmas proving global relations between various kinds of ast-bigblocks and cfg-blocks\<close>
+
+text \<open>'ending', 'ending2' and 'correctness_propagates_through_assumption' are helper lemmas 
+       used to complete the proofs of the global lemmas for ast-bigblocks, which are heads of loops. 
+       'ending2' and 'correctness_propagates_through_assumption' are used in the case where 
+       we're proving a global lemma for the head of a loop that is followed by another loop (not nested).\<close>
+lemma ending:
+  assumes "j = Suc j'" 
+      and "A,M,\<Lambda>,\<Gamma>,\<Omega>,T \<turnstile>(BigBlock None [] None None, KEndBlock (KSeq bigblock_next KStop), Normal ns1'') -n\<longrightarrow>^j' (reached_bb, reached_cont, reached_state)" 
+      and "\<And>m3 s3. (A,M,\<Lambda>,\<Gamma>,\<Omega>,G \<turnstile>(Inl n, Normal ns1'') -n\<rightarrow>* (m3, s3)) \<Longrightarrow> s3 \<noteq> Failure"
+      and "A,\<Lambda>,\<Gamma>,\<Omega> \<turnstile> \<langle>guard,ns1''\<rangle> \<Down> BoolV False" 
+      and "\<And> j''. 
+            j' = Suc (Suc j'') \<Longrightarrow>
+            A,M,\<Lambda>,\<Gamma>,\<Omega>,T \<turnstile>(bigblock_next, KStop, Normal ns1'') -n\<longrightarrow>^j'' (reached_bb, reached_cont, reached_state) \<Longrightarrow>
+           (\<And>m' s'. A,M,\<Lambda>,\<Gamma>,\<Omega>,G \<turnstile>(Inl n, Normal ns1'') -n\<rightarrow>* (m', s') \<Longrightarrow> s' \<noteq> Failure) \<Longrightarrow>
+           (A,\<Lambda>,\<Gamma>,\<Omega> \<turnstile> \<langle>UnOp Not guard,ns1''\<rangle> \<Down> BoolV True) \<Longrightarrow> (valid_configuration A \<Lambda> \<Gamma> \<Omega> [] reached_bb reached_cont reached_state)"
+    shows "valid_configuration A \<Lambda> \<Gamma> \<Omega> [] reached_bb reached_cont reached_state"
+proof -
+  from assms(2) have disj_a:
+    "(valid_configuration A \<Lambda> \<Gamma> \<Omega> [] reached_bb reached_cont reached_state) \<or> 
+       (\<exists> l2. (A,M,\<Lambda>,\<Gamma>,\<Omega>,T \<turnstile>(bigblock_next, KStop, Normal ns1'') -n\<longrightarrow>^l2 (reached_bb, reached_cont, reached_state)) \<and> (j' = Suc (Suc l2)) )" 
+    by (simp add: endblock_skip)
+  thus ?thesis
+  proof cases
+    assume "(valid_configuration A \<Lambda> \<Gamma> \<Omega> [] reached_bb reached_cont reached_state)" thus ?thesis by simp
+  next 
+    assume "\<not> ((valid_configuration A \<Lambda> \<Gamma> \<Omega> [] reached_bb reached_cont reached_state))"
+    hence "(\<exists> l2. (A,M,\<Lambda>,\<Gamma>,\<Omega>,T \<turnstile>(bigblock_next, KStop, Normal ns1'') -n\<longrightarrow>^l2 (reached_bb, reached_cont, reached_state)) \<and> (j' = Suc (Suc l2)) )" 
+      using disj_a by blast
+    thus ?thesis
+    proof -
+      obtain l2_conc where conc_trace: "(A,M,\<Lambda>,\<Gamma>,\<Omega>,T \<turnstile>(bigblock_next, KStop, Normal ns1'') -n\<longrightarrow>^l2_conc (reached_bb, reached_cont, reached_state))" and 
+                           succ_rel: "(j' = Suc (Suc l2_conc))"
+        using \<open>\<exists>l2. (A,M,\<Lambda>,\<Gamma>,\<Omega>,T \<turnstile>(bigblock_next, KStop, Normal ns1'') -n\<longrightarrow>^l2 (reached_bb, reached_cont, reached_state)) \<and> j' = Suc (Suc l2)\<close> by blast
+      show ?thesis
+        apply (rule assms(5))
+           apply (rule succ_rel)
+          apply (rule conc_trace)
+         apply (rule assms(3))
+         apply (simp)
+        using assms(4) false_equals_not_true 
+        by blast
+    qed
+  qed
+qed
+
+lemma correctness_propagates_through_assumption:
+  assumes "\<forall>m s. (A,M,\<Lambda>,\<Gamma>,\<Omega>,G \<turnstile>(Inl n0, Normal ns1) -n\<rightarrow>* (m, s)) \<longrightarrow> s \<noteq> Failure"
+      and "node_to_block G ! n0 = [Assume c]"
+      and "UnOp Not guard \<sim> c"
+      and "A,\<Lambda>,\<Gamma>,\<Omega> \<turnstile> \<langle>guard, ns1\<rangle> \<Down> BoolV False"
+      and "List.member (out_edges G ! n0) n1"
+    shows "\<And> m s. (A,M,\<Lambda>,\<Gamma>,\<Omega>,G \<turnstile>(Inl n1, Normal ns1) -n\<rightarrow>* (m, s)) \<Longrightarrow> s \<noteq> Failure"
+proof -
+  fix m1 s1
+  have "A,\<Lambda>,\<Gamma>,\<Omega> \<turnstile> \<langle>c, ns1\<rangle> \<Down> BoolV True" using assms(3-4) equiv_preserves_value false_equals_not_true by blast
+  then have a1: "(A,M,\<Lambda>,\<Gamma>,\<Omega> \<turnstile> \<langle>[Assume c], Normal ns1\<rangle> [\<rightarrow>] (Normal ns1))" by (meson RedAssumeOk RedCmdListCons RedCmdListNil)
+  show "(A,M,\<Lambda>,\<Gamma>,\<Omega>,G \<turnstile>(Inl n1, Normal ns1) -n\<rightarrow>* (m1, s1)) \<Longrightarrow> s1 \<noteq> Failure" 
+  proof -
+    assume "(A,M,\<Lambda>,\<Gamma>,\<Omega>,G \<turnstile>(Inl n1, Normal ns1) -n\<rightarrow>* (m1, s1))"
+    thus "s1 \<noteq> Failure" using a1 assms(1-2) assms(5) dag_verifies_propagate by blast 
+  qed
+qed
+
+lemma ending2:
+  assumes "j = Suc j'"
+      and "A,M,\<Lambda>,\<Gamma>,\<Omega>,T \<turnstile>(BigBlock None [] None None,
+                      KEndBlock (KSeq (BigBlock None [] (Some (WhileWrapper (ParsedWhile next_guard next_invs (next_body_bb#body_bbs)))) None) cont1),
+                      Normal ns1'') -n\<longrightarrow>^j'
+           (reached_bb, reached_cont, reached_state)"
+      and corr: "\<forall>m3 s3. (A,M,\<Lambda>,\<Gamma>,\<Omega>,G \<turnstile>(Inl n, Normal ns1'') -n\<rightarrow>* (m3, s3)) \<longrightarrow> s3 \<noteq> Failure"
+      and guard_false: "A,\<Lambda>,\<Gamma>,\<Omega> \<turnstile> \<langle>guard, ns1''\<rangle> \<Down> BoolV False" 
+      and "node_to_block G ! n = [Assume c]" 
+      and "(UnOp Not guard) \<sim> c"
+      and "List.member (out_edges(G) ! n) n1"
+      and "\<And> j'''.
+          j' = Suc (Suc (Suc j''')) \<Longrightarrow>
+          node_to_block G ! n = [Assume c] \<Longrightarrow>
+          (UnOp Not guard) \<sim> c \<Longrightarrow>
+          List.member (out_edges(G) ! n) n1 \<Longrightarrow>
+          A,M,\<Lambda>,\<Gamma>,\<Omega>,T \<turnstile>((BigBlock None [] (Some (ParsedWhile next_guard next_invs (next_body_bb#body_bbs))) None), KEndBlock cont1, Normal ns1'') -n\<longrightarrow>^j''' 
+              (reached_bb, reached_cont, reached_state) \<Longrightarrow>
+          (\<And>m' s'. A,M,\<Lambda>,\<Gamma>,\<Omega>,G \<turnstile>(Inl n1, Normal ns1'') -n\<rightarrow>* (m', s') \<Longrightarrow> s' \<noteq> Failure) \<Longrightarrow> 
+          (Ast.valid_configuration A \<Lambda> \<Gamma> \<Omega> [] reached_bb reached_cont reached_state)"
+    shows "(Ast.valid_configuration A \<Lambda> \<Gamma> \<Omega> [] reached_bb reached_cont reached_state)"
+  using assms
+proof -
+  from assms(2) have disj_a:
+    "(valid_configuration A \<Lambda> \<Gamma> \<Omega> [] reached_bb reached_cont reached_state) \<or> 
+       (\<exists> l3. (A,M,\<Lambda>,\<Gamma>,\<Omega>,T \<turnstile> ((BigBlock None [] (Some (ParsedWhile next_guard next_invs (next_body_bb#body_bbs))) None), KEndBlock cont1, Normal ns1'') 
+              -n\<longrightarrow>^l3 (reached_bb, reached_cont, reached_state)) \<and> (j' = Suc (Suc (Suc l3))) )"
+    by (simp add: endblock_skip_wrapper)
+  thus ?thesis
+  proof cases
+    assume "(valid_configuration A \<Lambda> \<Gamma> \<Omega> [] reached_bb reached_cont reached_state)" thus ?thesis by simp
+  next 
+    assume "\<not> ((valid_configuration A \<Lambda> \<Gamma> \<Omega> [] reached_bb reached_cont reached_state))"
+    hence skipped_endblock: 
+                  "(\<exists> l3. (A,M,\<Lambda>,\<Gamma>,\<Omega>,T \<turnstile>((BigBlock None [] (Some (ParsedWhile next_guard next_invs (next_body_bb#body_bbs))) None), KEndBlock cont1, Normal ns1'') 
+                   -n\<longrightarrow>^l3 (reached_bb, reached_cont, reached_state)) \<and> (j' = Suc (Suc (Suc l3))) )" 
+      using disj_a by blast
+    thus ?thesis
+    proof -
+      obtain l3_conc where 
+           conc_trace: "(A,M,\<Lambda>,\<Gamma>,\<Omega>,T \<turnstile>((BigBlock None [] (Some (ParsedWhile next_guard next_invs (next_body_bb#body_bbs))) None), KEndBlock cont1, Normal ns1'') 
+                        -n\<longrightarrow>^l3_conc (reached_bb, reached_cont, reached_state))" and 
+           succ_rel: "(j' = Suc (Suc (Suc l3_conc))) " 
+        using skipped_endblock by blast
+      show ?thesis
+        apply (rule assms(8))
+             apply (rule succ_rel)
+            apply (simp add: assms)
+           apply (rule assms(6))
+          apply (rule assms(7))
+         apply (rule conc_trace)
+        apply (rule correctness_propagates_through_assumption)
+             apply (rule corr)
+            apply (rule assms(5))
+           apply (rule assms(6))
+          apply (rule guard_false)
+         apply (rule assms(7))
+        apply simp
+        done
+    qed
+  qed
+qed
+
+text \<open>Global lemma for an ast-bigblock with a non-empty set of simple commands which concludes the program and is immediately after a loop.\<close>
+lemma generic_ending_block_after_loop_global_rel:
+  assumes syn_rel: "ast_cfg_rel None [] (BigBlock name cs1 None any_tr) cs2"
+  and "(any_tr = None) \<or> (any_tr = (Some (Return val1)))"
+  and "cs1 \<noteq> Nil"
+  and "cs2 \<noteq> Nil"
+  and "node_to_block G ! n = (c#cs2)" 
+  and "c = Assume b"
+  and "(UnOp Not guard) \<sim> b"
+  and trace_is_possible: "A,\<Lambda>,\<Gamma>,\<Omega> \<turnstile> \<langle>UnOp Not guard, ns1\<rangle> \<Down> BoolV True"
+  and j_step_ast_trace: "A,M,\<Lambda>,\<Gamma>,\<Omega>,T \<turnstile> ((BigBlock name cs1 None any_tr), KStop, (Normal ns1)) -n\<longrightarrow>^j (reached_bb, reached_cont, reached_state)"
+  and cfg_is_correct: "\<And> m' s'. (red_cfg_multi A M \<Lambda> \<Gamma> \<Omega> G ((Inl n),(Normal ns1)) (m',s')) \<Longrightarrow> (s' \<noteq> Failure)"
+  shows "(valid_configuration A \<Lambda> \<Gamma> \<Omega> [] reached_bb reached_cont reached_state)" 
+  using assms
+proof (cases j)
+  case 0
+  from this j_step_ast_trace have "(reached_bb, reached_cont, reached_state) = ((BigBlock name cs1 None any_tr), KStop, (Normal ns1))" by simp
+  then show ?thesis by (simp add: valid_configuration_def expr_all_sat_def)
+next
+  case (Suc j')
+  from this j_step_ast_trace obtain inter_bb inter_cont inter_state where
+    step: "A,M,\<Lambda>,\<Gamma>,\<Omega>,T \<turnstile> \<langle>((BigBlock name cs1 None any_tr), KStop, (Normal ns1))\<rangle> \<longrightarrow> (inter_bb, inter_cont, inter_state)" and
+    rest: "A,M,\<Lambda>,\<Gamma>,\<Omega>,T \<turnstile> (inter_bb, inter_cont, inter_state) -n\<longrightarrow>^j' (reached_bb, reached_cont, reached_state)"
+    by (metis prod_cases3 relpowp_Suc_D2) 
+  then show ?thesis 
+  proof (cases any_tr)
+    case None
+    from step this have concrete_inter: "(inter_bb, inter_cont, inter_state) = (BigBlock name [] None None, KStop, inter_state)"
+    proof cases
+      case RedSimpleCmds thus ?thesis using None by (auto simp add: RedSimpleCmds)
+    qed auto
+
+    have Red_impl: "(\<And> s2'.((red_cmd_list A M \<Lambda> \<Gamma> \<Omega> (c#cs2) (Normal ns1) s2') \<Longrightarrow> (s2' \<noteq> Failure)))" 
+      using dag_verifies_propagate_2  assms(5) cfg_is_correct by blast 
+
+    from step have "inter_state \<noteq> Failure"
+    proof cases
+      case RedSimpleCmds thus ?thesis using Red_impl trace_is_possible
+        by (metis assms(4) assms(7) assms(6) block_local_rel_guard_false step syn_rel)
+    qed auto
+
+    hence valid_inter: "(valid_configuration A \<Lambda> \<Gamma> \<Omega> [] inter_bb inter_cont inter_state)" 
+      unfolding valid_configuration_def expr_all_sat_def
+      using concrete_inter get_state.simps is_final.simps by simp
+
+    have "is_final (inter_bb, inter_cont, inter_state)" using concrete_inter by simp 
+    then show ?thesis by (metis Pair_inject concrete_inter final_is_static_propagate relpowp_imp_rtranclp rest valid_inter)
+  next
+    case (Some transfer)
+    then show ?thesis
+    proof (cases transfer)
+      case (Goto x1)
+      then show ?thesis using Some assms(2) by blast
+    next
+      case (Return ret)
+      from step this Some have concrete_inter: "(inter_bb, inter_cont, inter_state) = (BigBlock name [] None (Some (Return ret)), KStop, inter_state)"
+      proof cases
+        case RedSimpleCmds thus ?thesis using Return Some by blast
+      qed (auto simp add: assms(3))
+  
+      have Red_impl: "(\<And> s2'.((red_cmd_list A M \<Lambda> \<Gamma> \<Omega> (c#cs2) (Normal ns1) s2') \<Longrightarrow> (s2' \<noteq> Failure)))" 
+        using dag_verifies_propagate_2  assms(5) cfg_is_correct by blast 
+  
+      from step have "inter_state \<noteq> Failure"
+      proof cases
+        case RedSimpleCmds thus ?thesis using Red_impl trace_is_possible
+          by (metis assms(4) assms(7) assms(6) block_local_rel_guard_false step syn_rel)
+      qed auto
+      then show ?thesis 
+      proof (cases inter_state)
+        case (Normal x1)
+        then show ?thesis
+        proof (cases j')
+          case 0
+          then show ?thesis using concrete_inter by (metis Ast.valid_configuration_def \<open>inter_state \<noteq> Failure\<close> get_state.simps is_final.simps(4) relpowp_0_E rest)
+        next
+          case (Suc j'')
+          from this rest obtain inter_bb2 inter_cont2 inter_state2 where
+            snd_step: "A,M,\<Lambda>,\<Gamma>,\<Omega>,T \<turnstile> \<langle>(inter_bb, inter_cont, inter_state)\<rangle> \<longrightarrow> (inter_bb2, inter_cont2, inter_state2)" and
+            snd_rest: "A,M,\<Lambda>,\<Gamma>,\<Omega>,T \<turnstile> (inter_bb2, inter_cont2, inter_state2) -n\<longrightarrow>^j'' (reached_bb, reached_cont, reached_state)"
+            by (metis get_state.cases relpowp_Suc_E2)
+          then have inter2_conc: "(inter_bb2, inter_cont2, inter_state2) = ((BigBlock name [] None None), KStop, inter_state)" 
+            using concrete_inter \<open>inter_state \<noteq> Failure\<close> Normal
+          proof cases
+            case RedReturn thus ?thesis using concrete_inter \<open>inter_state \<noteq> Failure\<close> Normal by blast
+          qed auto
+          hence "is_final (inter_bb2, inter_cont2, inter_state2)" by simp
+          then show ?thesis
+            by (metis Ast.valid_configuration_def inter2_conc \<open>inter_state \<noteq> Failure\<close> expr_all_sat_def final_is_static_propagate get_state.simps list.pred_inject(1) rtranclp_power snd_rest)
+        qed
+      next
+        case Failure
+        then show ?thesis using \<open>inter_state \<noteq> Failure\<close> by simp
+      next
+        case Magic
+        then show ?thesis by (metis Ast.valid_configuration_def \<open>inter_state \<noteq> Failure\<close> get_state.simps magic_propagates rest state.simps(5))
+      qed
+    qed
+  qed
+qed
+
+
+text \<open>Global lemma for an ast-bigblock with a non-empty set of simple commands which concludes the program.\<close>
+lemma generic_ending_block_global_rel:
+  assumes syn_rel: "ast_cfg_rel None [] (BigBlock name cs1 None any_tr) cs2"
+  and j_step_ast_trace: "A,M,\<Lambda>,\<Gamma>,\<Omega>,T \<turnstile> ((BigBlock name cs1 None any_tr), KStop, (Normal ns1)) -n\<longrightarrow>^j (reached_bb, reached_cont, reached_state)"
+  and "(any_tr = None) \<or> (any_tr = (Some (Return val1)))"
+  and "cs1 \<noteq> Nil"
+  and "cs2 \<noteq> Nil"
+  and "node_to_block G ! n = cs2"
+  and cfg_is_correct: "\<And> m' s'. (red_cfg_multi A M \<Lambda> \<Gamma> \<Omega> G ((Inl n),(Normal ns1)) (m',s')) \<Longrightarrow> (s' \<noteq> Failure)" 
+shows "(valid_configuration A \<Lambda> \<Gamma> \<Omega> [] reached_bb reached_cont reached_state)"
+  using assms
+proof (cases j)
+  case 0
+  from this j_step_ast_trace have "(reached_bb, reached_cont, reached_state) = ((BigBlock name cs1 None any_tr), KStop, (Normal ns1))" by simp
+  then show ?thesis by (simp add: valid_configuration_def expr_all_sat_def)
+next
+  case (Suc j')
+  from this j_step_ast_trace obtain inter_bb inter_cont inter_state where
+    step: "A,M,\<Lambda>,\<Gamma>,\<Omega>,T \<turnstile> \<langle>((BigBlock name cs1 None any_tr), KStop, (Normal ns1))\<rangle> \<longrightarrow> (inter_bb, inter_cont, inter_state)" and
+    rest: "A,M,\<Lambda>,\<Gamma>,\<Omega>,T \<turnstile> (inter_bb, inter_cont, inter_state) -n\<longrightarrow>^j' (reached_bb, reached_cont, reached_state)"
+    by (metis prod_cases3 relpowp_Suc_D2) 
+  then show ?thesis 
+  proof (cases any_tr)
+    case None
+    from step this have concrete_inter: "(inter_bb, inter_cont, inter_state) = (BigBlock name [] None None, KStop, inter_state)"
+    proof cases
+      case RedSimpleCmds thus ?thesis using None by (auto simp add: RedSimpleCmds)
+    qed auto
+
+    have Red_impl: "(\<And> s2'.((red_cmd_list A M \<Lambda> \<Gamma> \<Omega> cs2 (Normal ns1) s2') \<Longrightarrow> (s2' \<noteq> Failure)))"
+      using assms(6) cfg_is_correct dag_verifies_propagate_2 by blast
+
+    from step have "inter_state \<noteq> Failure"
+    proof cases
+      case RedSimpleCmds thus ?thesis using Red_impl assms(5) block_local_rel_generic local.step syn_rel by blast
+    qed auto
+
+    hence valid_inter: "(valid_configuration A \<Lambda> \<Gamma> \<Omega> [] inter_bb inter_cont inter_state)" 
+      unfolding valid_configuration_def expr_all_sat_def
+      using concrete_inter get_state.simps is_final.simps by simp
+
+    have "is_final (inter_bb, inter_cont, inter_state)" using concrete_inter by simp 
+    then show ?thesis by (metis Pair_inject concrete_inter final_is_static_propagate relpowp_imp_rtranclp rest valid_inter)
+  next
+    case (Some transfer)
+    then show ?thesis
+    proof (cases transfer)
+      case (Goto x1)
+      then show ?thesis using Some assms(3) by blast
+    next
+      case (Return ret)
+      from step this Some have concrete_inter: "(inter_bb, inter_cont, inter_state) = (BigBlock name [] None (Some (Return ret)), KStop, inter_state)"
+      proof cases
+        case RedSimpleCmds thus ?thesis using Return Some by blast
+      qed (auto simp add: assms(4))
+  
+      have Red_impl: "(\<And> s2'.((red_cmd_list A M \<Lambda> \<Gamma> \<Omega> cs2 (Normal ns1) s2') \<Longrightarrow> (s2' \<noteq> Failure)))" 
+        using dag_verifies_propagate_2  assms(6) cfg_is_correct by blast 
+  
+      from step have "inter_state \<noteq> Failure"
+      proof cases
+        case RedSimpleCmds thus ?thesis using Red_impl using assms(5) block_local_rel_generic local.step syn_rel by blast
+      qed auto
+
+      then show ?thesis
+      proof (cases inter_state)
+        case (Normal x1)
+        then show ?thesis
+        proof (cases j')
+          case 0
+          then show ?thesis using concrete_inter by (metis Ast.valid_configuration_def \<open>inter_state \<noteq> Failure\<close> get_state.simps is_final.simps(4) relpowp_0_E rest)
+        next
+          case (Suc j'')
+          from this rest obtain inter_bb2 inter_cont2 inter_state2 where
+            snd_step: "A,M,\<Lambda>,\<Gamma>,\<Omega>,T \<turnstile> \<langle>(inter_bb, inter_cont, inter_state)\<rangle> \<longrightarrow> (inter_bb2, inter_cont2, inter_state2)" and
+            snd_rest: "A,M,\<Lambda>,\<Gamma>,\<Omega>,T \<turnstile> (inter_bb2, inter_cont2, inter_state2) -n\<longrightarrow>^j'' (reached_bb, reached_cont, reached_state)"
+            by (metis get_state.cases relpowp_Suc_E2)
+          then have inter2_conc: "(inter_bb2, inter_cont2, inter_state2) = ((BigBlock name [] None None), KStop, inter_state)" 
+            using concrete_inter \<open>inter_state \<noteq> Failure\<close> Normal
+          proof cases
+            case RedReturn thus ?thesis using concrete_inter \<open>inter_state \<noteq> Failure\<close> Normal by blast
+          qed auto
+          hence "is_final (inter_bb2, inter_cont2, inter_state2)" by simp
+          then show ?thesis
+            by (metis Ast.valid_configuration_def inter2_conc \<open>inter_state \<noteq> Failure\<close> expr_all_sat_def final_is_static_propagate get_state.simps list.pred_inject(1) rtranclp_power snd_rest)
+        qed
+      next
+        case Failure
+        then show ?thesis using \<open>inter_state \<noteq> Failure\<close> by simp
+      next
+        case Magic
+        then show ?thesis by (metis valid_configuration_def \<open>inter_state \<noteq> Failure\<close> get_state.simps magic_propagates rest state.simps(5))
+      qed
+    qed
+  qed
+qed
+
+
+text \<open>Global lemma for an ast-bigblock with a non-empty set of simple commands that enters a loop after it executes its simple cmds.\<close>
+lemma block_global_rel_while_successor:
+  assumes j_step_ast_trace: 
+      "A,M,\<Lambda>,\<Gamma>,\<Omega>,T \<turnstile> ((BigBlock name cmds (Some (WhileWrapper (ParsedWhile guard invs (body_bb0#body_bbs)))) None), cont1, Normal ns1) -n\<longrightarrow>^j 
+                      (reached_bb, reached_cont, reached_state)"
+  and syn_rel: "ast_cfg_rel None [] (BigBlock name cmds (Some (WhileWrapper (ParsedWhile guard invs (body_bb0#body_bbs)))) None) cmds"
+  and "cmds \<noteq> []"
+  and "node_to_block G ! n = cmds"
+  and cfg_is_correct: "\<And> m' s'. (red_cfg_multi A M \<Lambda> \<Gamma> \<Omega> G ((Inl n),(Normal ns1)) (m',s')) \<Longrightarrow> (s' \<noteq> Failure)"
+  and block_local_rel:
+    "\<And> reached_bb_inter reached_cont_inter reached_state_inter. 
+    (red_bigblock A M \<Lambda> \<Gamma> \<Omega> T ((BigBlock name cmds (Some (WhileWrapper (ParsedWhile guard invs (body_bb0#body_bbs)))) None), cont1, (Normal ns1)) (reached_bb_inter, reached_cont_inter, reached_state_inter)) \<Longrightarrow> 
+    (\<And> s2'.((red_cmd_list A M \<Lambda> \<Gamma> \<Omega> cmds (Normal ns1) s2') \<Longrightarrow> (s2' \<noteq> Failure))) \<Longrightarrow>   
+    (reached_state_inter \<noteq> Failure  \<and> (\<forall>ns1'. reached_state_inter = Normal ns1' \<longrightarrow> (A,M,\<Lambda>,\<Gamma>,\<Omega> \<turnstile> \<langle>cmds, Normal ns1\<rangle> [\<rightarrow>] Normal ns1')))"
+  and global_rel_succ:
+        "\<And> ns2 k.
+         k < j \<Longrightarrow>
+         (\<forall>msuc2. List.member (out_edges(G) ! n) msuc2 \<longrightarrow> (\<forall>m3 s3. (A,M,\<Lambda>,\<Gamma>,\<Omega>,G \<turnstile> (Inl msuc2, Normal ns2) -n\<rightarrow>* (m3, s3)) \<longrightarrow> s3 \<noteq> Failure)) \<Longrightarrow>
+         A,M,\<Lambda>,\<Gamma>,\<Omega>,T \<turnstile> ((BigBlock name [] (Some (ParsedWhile guard invs (body_bb0#body_bbs))) None), KEndBlock cont1, Normal ns2) -n\<longrightarrow>^k 
+                      (reached_bb, reached_cont, reached_state) \<Longrightarrow> 
+         (valid_configuration A \<Lambda> \<Gamma> \<Omega> [] reached_bb reached_cont reached_state)"
+  shows "(valid_configuration A \<Lambda> \<Gamma> \<Omega> [] reached_bb reached_cont reached_state)"
+  using assms
+proof cases
+  assume "j = 0"
+  then have "(reached_bb, reached_cont, reached_state) = 
+             ((BigBlock name cmds (Some (WhileWrapper (ParsedWhile guard invs (body_bb0#body_bbs)))) None), cont1, Normal ns1)" using j_step_ast_trace by auto
+  thus ?thesis by (simp add: valid_configuration_def)
+next
+  assume "j \<noteq> 0"
+  from this obtain j' where "j = Suc j'" using not0_implies_Suc by blast
+  from this j_step_ast_trace obtain inter_bb inter_cont inter_state where
+    first_step: "A,M,\<Lambda>,\<Gamma>,\<Omega>,T \<turnstile> \<langle>((BigBlock name cmds (Some (WhileWrapper (ParsedWhile guard invs (body_bb0#body_bbs)))) None), cont1, Normal ns1)\<rangle> \<longrightarrow> (inter_bb, inter_cont, inter_state)" and 
+    rest: "A,M,\<Lambda>,\<Gamma>,\<Omega>,T \<turnstile> (inter_bb, inter_cont, inter_state) -n\<longrightarrow>^j' (reached_bb, reached_cont, reached_state)"
+    by (metis (no_types, opaque_lifting) get_state.cases relpowp_Suc_D2)
+  from this have a1: "(inter_bb, inter_cont, inter_state) = ((BigBlock name [] (Some (WhileWrapper (ParsedWhile guard invs (body_bb0#body_bbs)))) None), cont1, inter_state)"
+  proof cases
+    case RedSimpleCmds thus ?thesis by blast
+  qed (auto simp add: \<open>cmds \<noteq> []\<close>)
+  have Red_impl: "(\<And> s2'.((red_cmd_list A M \<Lambda> \<Gamma> \<Omega> cmds (Normal ns1) s2') \<Longrightarrow> (s2' \<noteq> Failure)))" using dag_verifies_propagate_2 cfg_is_correct assms(4) by blast
+  have local_conclusion: "inter_state \<noteq> Failure  \<and> (\<forall>ns1'. inter_state = Normal ns1' \<longrightarrow> (A,M,\<Lambda>,\<Gamma>,\<Omega> \<turnstile> \<langle>cmds, Normal ns1\<rangle> [\<rightarrow>] Normal ns1'))" 
+    using Red_impl first_step assms(3) block_local_rel_generic syn_rel by blast 
+  show ?thesis 
+  proof (cases inter_state)
+    case (Normal x1)
+    hence "(A,M,\<Lambda>,\<Gamma>,\<Omega> \<turnstile> \<langle>cmds, Normal ns1\<rangle> [\<rightarrow>] inter_state)" using local_conclusion by blast
+    then show ?thesis
+    proof (cases j')
+      case 0
+      then show ?thesis 
+        by (metis (full_types, opaque_lifting) Ast.valid_configuration_def expr_all_sat_def get_state.simps list.pred_inject(1) local_conclusion relpowp.simps(1) rest)
+    next
+      case 2: (Suc j'')
+
+      hence Red_cfg_conc: 
+        "(\<forall>msuc2. List.member (out_edges(G) ! n) msuc2 \<longrightarrow> (\<forall>m3 s3. (A,M,\<Lambda>,\<Gamma>,\<Omega>,G \<turnstile> (Inl msuc2, inter_state) -n\<rightarrow>* (m3, s3)) \<longrightarrow> s3 \<noteq> Failure))" 
+        using dag_verifies_propagate Normal \<open>A,M,\<Lambda>,\<Gamma>,\<Omega> \<turnstile> \<langle>cmds,Normal ns1\<rangle> [\<rightarrow>] inter_state\<close> assms(4) cfg_is_correct 
+        by blast
+
+      from 2 j_step_ast_trace obtain inter_bb2 inter_cont2 inter_state2 where
+        first_step_2: "A,M,\<Lambda>,\<Gamma>,\<Omega>,T \<turnstile> \<langle>(inter_bb, inter_cont, inter_state)\<rangle> \<longrightarrow> (inter_bb2, inter_cont2, inter_state2)" and 
+        rest_2: "A,M,\<Lambda>,\<Gamma>,\<Omega>,T \<turnstile> (inter_bb2, inter_cont2, inter_state2) -n\<longrightarrow>^j'' (reached_bb, reached_cont, reached_state)"
+        by (metis get_state.cases relpowp_Suc_E2 rest)
+      from this have a3: "(inter_bb2, inter_cont2, inter_state2) = 
+                          ((BigBlock name [] (Some (ParsedWhile guard invs (body_bb0#body_bbs))) None), KEndBlock cont1, inter_state)"
+        using a1 Normal
+      proof cases
+        case RedParsedWhileWrapper thus ?thesis using a1 by fastforce
+      qed auto 
+
+      have "j'' < j" by (simp add: "2" \<open>j = Suc j'\<close>)
+      then show ?thesis using a3 rest_2 Normal Red_cfg_conc assms(7) by blast
+    qed
+  next
+    case Failure
+    then show ?thesis using local_conclusion by blast
+  next
+    case Magic
+    then show ?thesis by (metis valid_configuration_def get_state.simps local_conclusion magic_propagates rest state.simps(5))
+  qed
+qed
+
+text \<open>Global lemma for a loop-head ast-bigblock with non-empty invariants. The loop is also required to be non-empty.\<close>
+lemma block_global_rel_loop_head:
+  assumes block_rel: "ast_cfg_rel None assertions (BigBlock name [] any_str any_tr) assertions"
+  and ast_trace: "A,M,\<Lambda>,\<Gamma>,\<Omega>,T \<turnstile> ((BigBlock name [] any_str any_tr), KEndBlock cont1, (Normal ns1)) -n\<longrightarrow>^j (reached_bb, reached_cont, reached_state)"
+  and cfg_correct: "(\<And> m2 s2. ((red_cfg_multi A M \<Lambda> \<Gamma> \<Omega> G (Inl n, Normal ns1) (m2, s2)) \<Longrightarrow> (s2 \<noteq> Failure)))"
+  (* TODO: You're requiring that the loop isn't empty! What if it is? *)
+  and bb_successor_while: "any_str = Some (ParsedWhile cont_guard invs (bb0#body_bbs))"
+  and block_local_rel:
+    "\<And> reached_bb_inter reached_cont_inter reached_state_inter. (red_bigblock A M \<Lambda> \<Gamma> \<Omega> T ((BigBlock name [] any_str any_tr), KEndBlock cont1, (Normal ns1)) (reached_bb_inter, reached_cont_inter, reached_state_inter)) \<Longrightarrow> 
+    (\<And> s2'.((red_cmd_list A M \<Lambda> \<Gamma> \<Omega> assertions (Normal ns1) s2') \<Longrightarrow> (s2' \<noteq> Failure))) \<Longrightarrow>   
+    (reached_state_inter \<noteq> Failure  \<and> (\<forall>ns1'. reached_state_inter = Normal ns1' \<longrightarrow> (A,M,\<Lambda>,\<Gamma>,\<Omega> \<turnstile> \<langle>assertions, Normal ns1\<rangle> [\<rightarrow>] Normal ns1')))"
+  (* TODO: The following is a sketchy assumption! Fix it!*)
+  and "assertions \<noteq> []" 
+  and "node_to_block(G) ! n = assertions"
+  and succ_correct: 
+   "\<And> ns1'' loop_guard j'. 
+    j = Suc j' \<Longrightarrow>
+    (\<forall>msuc2.  List.member (out_edges(G) ! n) msuc2 \<longrightarrow> (\<forall>m3 s3. ((A,M,\<Lambda>,\<Gamma>,\<Omega>,G \<turnstile> (Inl(msuc2), Normal ns1'') -n\<rightarrow>* (m3, s3)) \<longrightarrow> s3 \<noteq> Failure))) \<Longrightarrow>
+    ((cont_guard = Some loop_guard) \<and> 
+      (red_expr A \<Lambda> \<Gamma> \<Omega> loop_guard ns1'' (BoolV True)) \<and> 
+      A,M,\<Lambda>,\<Gamma>,\<Omega>,T \<turnstile> (bb0, convert_list_to_cont (rev ((BigBlock name [] any_str any_tr)#body_bbs)) (KEndBlock cont1), (Normal ns1'')) -n\<longrightarrow>^j' (reached_bb, reached_cont, reached_state)) \<or> 
+    ((cont_guard = Some loop_guard) \<and> 
+      (red_expr A \<Lambda> \<Gamma> \<Omega> loop_guard ns1'' (BoolV False)) \<and> 
+      A,M,\<Lambda>,\<Gamma>,\<Omega>,T \<turnstile> ((BigBlock name [] None None), KEndBlock cont1, (Normal ns1'')) -n\<longrightarrow>^j' (reached_bb, reached_cont, reached_state)) \<or>
+    ((cont_guard = None) \<and> 
+     ((A,M,\<Lambda>,\<Gamma>,\<Omega>,T \<turnstile> ((BigBlock name [] None None), KEndBlock cont1, (Normal ns1'')) -n\<longrightarrow>^j' (reached_bb, reached_cont, reached_state)) \<or>
+      (A,M,\<Lambda>,\<Gamma>,\<Omega>,T \<turnstile> (bb0, convert_list_to_cont (rev ((BigBlock name [] any_str any_tr)#body_bbs)) (KEndBlock cont1), (Normal ns1'')) -n\<longrightarrow>^j' (reached_bb, reached_cont, reached_state))))  \<Longrightarrow>  
+    (Ast.valid_configuration A \<Lambda> \<Gamma> \<Omega> posts reached_bb reached_cont reached_state)"
+  shows "(Ast.valid_configuration A \<Lambda> \<Gamma> \<Omega> posts reached_bb reached_cont reached_state)" 
+  using assms
+proof cases
+    case (Rel_Invs)
+    thus ?thesis 
+    proof cases
+      assume "j = 0"
+      hence "(reached_bb, reached_cont, reached_state) = ((BigBlock name [] any_str any_tr), KEndBlock cont1, (Normal ns1))" using ast_trace by simp 
+      thus ?thesis by (simp add: Ast.valid_configuration_def)
+    next
+      assume "j \<noteq> 0" 
+      from this obtain j' where "j = Suc j'" using not0_implies_Suc by blast
+  
+      from ast_trace this obtain inter_bb inter_cont inter_state where
+        first_step: "A,M,\<Lambda>,\<Gamma>,\<Omega>,T \<turnstile> \<langle>((BigBlock name [] any_str any_tr), KEndBlock cont1, (Normal ns1))\<rangle> \<longrightarrow> (inter_bb, inter_cont, inter_state)" and
+        rest: "A,M,\<Lambda>,\<Gamma>,\<Omega>,T \<turnstile> (inter_bb, inter_cont, inter_state) -n\<longrightarrow>^j' (reached_bb, reached_cont, reached_state)"
+        by (metis prod_cases3 relpowp_Suc_D2)
+  
+      show ?thesis
+      proof (cases cont_guard)
+        case None
+        from first_step show ?thesis using bb_successor_while
+        proof cases
+          case RedParsedWhileTrue
+          hence concrete_inter1: "(inter_bb, inter_cont, inter_state) = (bb0, convert_list_to_cont (rev ((BigBlock name [] any_str any_tr)#body_bbs)) (KEndBlock cont1), (Normal ns1))"
+            using bb_successor_while None by blast
+  
+          from first_step
+          have succ_cfg_correct: "(\<forall>msuc2.  List.member (out_edges(G) ! n) msuc2 \<longrightarrow> (\<forall>m3 s3. ((A,M,\<Lambda>,\<Gamma>,\<Omega>,G \<turnstile> (Inl(msuc2), inter_state) -n\<rightarrow>* (m3, s3)) \<longrightarrow> s3 \<noteq> Failure)))"
+            by (metis Pair_inject assms(7) block_local_rel cfg_correct concrete_inter1 dag_verifies_propagate dag_verifies_propagate_2)
+  
+          show ?thesis using \<open>j = Suc j'\<close> succ_cfg_correct None rest concrete_inter1 succ_correct by blast 
+        next 
+          case RedParsedWhileFalse
+          hence concrete_inter2: "(inter_bb, inter_cont, inter_state) = ((BigBlock name [] None None), KEndBlock cont1, (Normal ns1))" by simp
+  
+          from first_step
+          have succ_cfg_correct: "(\<forall>msuc2.  List.member (out_edges(G) ! n) msuc2 \<longrightarrow> (\<forall>m3 s3. ((A,M,\<Lambda>,\<Gamma>,\<Omega>,G \<turnstile> (Inl(msuc2), inter_state) -n\<rightarrow>* (m3, s3)) \<longrightarrow> s3 \<noteq> Failure)))"
+            by (metis assms(7) block_local_rel cfg_correct dag_verifies_propagate dag_verifies_propagate_2 local.RedParsedWhileFalse(5))
+  
+          show ?thesis using \<open>j = Suc j'\<close> succ_cfg_correct None rest concrete_inter2 succ_correct by blast
+        next 
+          case RedParsedWhile_InvFail thus ?thesis using assms(7) block_local_rel cfg_correct dag_verifies_propagate_2 first_step by blast
+        qed auto
+      next
+        case (Some concrete_loop_guard)
+        then show ?thesis 
+        proof cases
+          assume guard_true: "(red_expr A \<Lambda> \<Gamma> \<Omega> concrete_loop_guard ns1 (BoolV True))"
+          hence guard_not_false: "\<not> (red_expr A \<Lambda> \<Gamma> \<Omega> concrete_loop_guard ns1 (BoolV False))" using expr_eval_determ by blast
+  
+          from first_step show ?thesis 
+          proof cases
+            case RedParsedWhileTrue
+            hence concrete_inter3: "(inter_bb, inter_cont, inter_state) = (bb0, convert_list_to_cont (rev ((BigBlock name [] any_str any_tr)#body_bbs)) (KEndBlock cont1), (Normal ns1))"
+              using bb_successor_while Some by blast
+  
+            from first_step
+            have succ_cfg_correct: "(\<forall>msuc2.  List.member (out_edges(G) ! n) msuc2 \<longrightarrow> (\<forall>m3 s3. ((A,M,\<Lambda>,\<Gamma>,\<Omega>,G \<turnstile> (Inl(msuc2), inter_state) -n\<rightarrow>* (m3, s3)) \<longrightarrow> s3 \<noteq> Failure)))"
+              by (metis Pair_inject assms(7) block_local_rel cfg_correct concrete_inter3 dag_verifies_propagate dag_verifies_propagate_2)
+  
+            show ?thesis using \<open>j = Suc j'\<close> succ_cfg_correct Some guard_true rest concrete_inter3 succ_correct by blast 
+        next 
+            case RedParsedWhile_InvFail thus ?thesis using assms(7) block_local_rel cfg_correct dag_verifies_propagate_2 first_step by blast
+        qed (auto simp add: bb_successor_while Some guard_not_false)
+      next
+        assume guard_not_true: "\<not> (red_expr A \<Lambda> \<Gamma> \<Omega> concrete_loop_guard ns1 (BoolV True))"
+        thus ?thesis 
+        proof cases
+          assume guard_false: "(red_expr A \<Lambda> \<Gamma> \<Omega> concrete_loop_guard ns1 (BoolV False))"
+  
+          from first_step show ?thesis 
+          proof cases
+            case RedParsedWhileFalse
+            hence concrete_inter4: "(inter_bb, inter_cont, inter_state) = ((BigBlock name [] None None), KEndBlock cont1, (Normal ns1))" by simp
+
+          from first_step
+          have succ_cfg_correct: "(\<forall>msuc2.  List.member (out_edges(G) ! n) msuc2 \<longrightarrow> (\<forall>m3 s3. ((A,M,\<Lambda>,\<Gamma>,\<Omega>,G \<turnstile> (Inl(msuc2), inter_state) -n\<rightarrow>* (m3, s3)) \<longrightarrow> s3 \<noteq> Failure)))"
+            by (metis assms(7) block_local_rel cfg_correct dag_verifies_propagate dag_verifies_propagate_2 local.RedParsedWhileFalse(5))
+  
+            show ?thesis using \<open>j = Suc j'\<close> succ_cfg_correct Some guard_false rest concrete_inter4 succ_correct by blast
+          next
+            case RedParsedWhile_InvFail thus ?thesis using Some bb_successor_while guard_not_true by blast
+          qed (auto simp add: bb_successor_while Some guard_not_true)
+        next
+          assume guard_not_false: "\<not> (red_expr A \<Lambda> \<Gamma> \<Omega> concrete_loop_guard ns1 (BoolV False))"
+          from first_step show ?thesis
+          proof cases
+            case RedParsedWhile_InvFail thus ?thesis using Some bb_successor_while guard_not_true by blast
+          qed (auto simp add: bb_successor_while Some guard_not_true guard_not_false)
+        qed
+      qed
+    qed
+  qed
+qed auto
+
+text \<open>Global lemma for an ast-bigblock with a non-empty set of simple cmds which enters an if-statement after executing its simple cmds.\<close>
+lemma block_global_rel_if_successor:
+  assumes block_rel: "ast_cfg_rel None [] (BigBlock name cs1 any_str any_tr) cs2"
+  and ast_trace: "A,M,\<Lambda>,\<Gamma>,\<Omega>,T \<turnstile> ((BigBlock name cs1 any_str any_tr), cont0, (Normal ns1)) -n\<longrightarrow>^j (reached_bb, reached_cont, reached_state)"
+  and "cs1 \<noteq> Nil"
+  and "cs2 \<noteq> Nil"
+  and "node_to_block(G) ! n = cs2"
+  and cfg_correct: "(\<And> m2 s2. ((red_cfg_multi A M \<Lambda> \<Gamma> \<Omega> G (Inl n, Normal ns1) (m2, s2)) \<Longrightarrow> (s2 \<noteq> Failure)))"
+  and bb_successor_if: "any_str = Some (ParsedIf cont_guard (then0#then_bbs) (else0#else_bbs))"
+  and block_local_rel:
+        "\<And> reached_bb_inter reached_cont_inter reached_state_inter. (red_bigblock A M \<Lambda> \<Gamma> \<Omega> T ((BigBlock name cs1 any_str any_tr), cont0, (Normal ns1)) (reached_bb_inter, reached_cont_inter, reached_state_inter)) \<Longrightarrow> 
+        (\<And> s2'.((red_cmd_list A M \<Lambda> \<Gamma> \<Omega> cs2 (Normal ns1) s2') \<Longrightarrow> (s2' \<noteq> Failure))) \<Longrightarrow>   
+        (reached_state_inter \<noteq> Failure  \<and> (\<forall>ns1'. reached_state_inter = Normal ns1' \<longrightarrow> (A,M,\<Lambda>,\<Gamma>,\<Omega> \<turnstile> \<langle>cs2, Normal ns1\<rangle> [\<rightarrow>] Normal ns1')))"
+  and succ_correct: 
+       "\<And> ns1'' block_guard k.
+         k < j \<Longrightarrow> 
+        (\<forall>msuc2.  List.member (out_edges(G) ! n) msuc2 \<longrightarrow> (\<forall>m3 s3. ((A,M,\<Lambda>,\<Gamma>,\<Omega>,G \<turnstile> (Inl(msuc2), Normal ns1'') -n\<rightarrow>* (m3, s3)) \<longrightarrow> s3 \<noteq> Failure))) \<Longrightarrow>
+        ((cont_guard = Some block_guard) \<and> 
+          (red_expr A \<Lambda> \<Gamma> \<Omega> block_guard ns1'' (BoolV True)) \<and> 
+          A,M,\<Lambda>,\<Gamma>,\<Omega>,T \<turnstile> (then0, convert_list_to_cont (rev then_bbs) cont0, (Normal ns1'')) -n\<longrightarrow>^k (reached_bb, reached_cont, reached_state)) \<or> 
+        ((cont_guard = Some block_guard) \<and> 
+          (red_expr A \<Lambda> \<Gamma> \<Omega> block_guard ns1'' (BoolV False)) \<and> 
+          A,M,\<Lambda>,\<Gamma>,\<Omega>,T \<turnstile> (else0, convert_list_to_cont (rev else_bbs) cont0, (Normal ns1'')) -n\<longrightarrow>^k (reached_bb, reached_cont, reached_state)) \<or>
+        ( (cont_guard = None) \<and> 
+          ((A,M,\<Lambda>,\<Gamma>,\<Omega>,T \<turnstile> (then0, convert_list_to_cont (rev then_bbs) cont0, (Normal ns1'')) -n\<longrightarrow>^k (reached_bb, reached_cont, reached_state)) \<or>
+          (A,M,\<Lambda>,\<Gamma>,\<Omega>,T \<turnstile> (else0, convert_list_to_cont (rev else_bbs) cont0, (Normal ns1'')) -n\<longrightarrow>^k (reached_bb, reached_cont, reached_state))) ) \<Longrightarrow>  
+        (Ast.valid_configuration A \<Lambda> \<Gamma> \<Omega> posts reached_bb reached_cont reached_state)"
+  shows "(Ast.valid_configuration A \<Lambda> \<Gamma> \<Omega> posts reached_bb reached_cont reached_state)" 
+  using assms
+proof cases
+  case Rel_Main_test
+  have not_end: "(cont0 \<noteq> KStop) \<or> any_str \<noteq> None \<or> any_tr \<noteq> None" using bb_successor_if by simp
+  from ast_trace show ?thesis
+  proof (cases j)
+    case 0
+    hence "(reached_bb, reached_cont, reached_state) = ((BigBlock name cs1 any_str any_tr), cont0, (Normal ns1))" using ast_trace by auto
+    then show ?thesis by (simp add: Ast.valid_configuration_def bb_successor_if) 
+  next
+    case 1: (Suc j')
+    from this obtain inter_bb inter_cont inter_state where
+      first_step: "red_bigblock A M \<Lambda> \<Gamma> \<Omega> T ((BigBlock name cs1 any_str any_tr), cont0, (Normal ns1)) (inter_bb, inter_cont, inter_state)" and
+      rest_of_steps: "A,M,\<Lambda>,\<Gamma>,\<Omega>,T \<turnstile> (inter_bb, inter_cont, inter_state) -n\<longrightarrow>^j' (reached_bb, reached_cont, reached_state)" 
+      by (metis ast_trace get_state.cases relpowp_Suc_E2)
+
+    from cfg_correct \<open>cs2 \<noteq> Nil\<close> \<open>node_to_block(G) ! n = cs2\<close> 
+    have local_rel_corr: "(\<And> s2'.((red_cmd_list A M \<Lambda> \<Gamma> \<Omega> (cs2) (Normal ns1) s2') \<Longrightarrow> (s2' \<noteq> Failure)))"
+      using dag_verifies_propagate_2 by blast
+
+    from local_rel_corr first_step 
+    have a2: "(inter_state \<noteq> Failure  \<and> (\<forall>ns1'. inter_state = Normal ns1' \<longrightarrow> (A,M,\<Lambda>,\<Gamma>,\<Omega> \<turnstile> \<langle>cs2, Normal ns1\<rangle> [\<rightarrow>] Normal ns1')))" 
+      using block_local_rel by simp
+
+    from first_step \<open>cs1 \<noteq> Nil\<close> 
+    have a1: "(inter_bb, inter_cont, inter_state) = ((BigBlock name [] any_str any_tr), cont0, inter_state)"
+    proof cases
+      case RedSimpleCmds then show ?thesis by (auto simp add: RedSimpleCmds)
+    qed auto
+
+    show ?thesis 
+    proof (cases inter_state)
+      case 2: (Normal x1)
+      from rest_of_steps show ?thesis 
+      proof (cases j')
+        case 0
+        then show ?thesis 
+          by (metis Ast.valid_configuration_def a1 a2 bb_successor_if get_state.simps is_final.simps(3) relpowp_0_E rest_of_steps) 
+      next
+        case 3: (Suc j'')
+        from this rest_of_steps obtain snd_inter_bb snd_inter_cont snd_inter_state where
+          snd_step: "red_bigblock A M \<Lambda> \<Gamma> \<Omega> T ((BigBlock name [] any_str any_tr), cont0, inter_state)  (snd_inter_bb, snd_inter_cont, snd_inter_state)" and
+          snd_rest_of_steps: "A,M,\<Lambda>,\<Gamma>,\<Omega>,T \<turnstile> (snd_inter_bb, snd_inter_cont, snd_inter_state) -n\<longrightarrow>^j'' (reached_bb, reached_cont, reached_state)"
+          by (metis a1 get_state.cases relpowp_Suc_D2)
+
+        thus ?thesis 
+        proof (cases cont_guard)
+          case None
+          from snd_step this show ?thesis
+          proof cases
+            case RedParsedIfTrue
+            hence eq: "(snd_inter_bb, snd_inter_cont, snd_inter_state) = (then0, convert_list_to_cont (rev then_bbs) cont0, inter_state)" using None bb_successor_if 1 by auto
+
+            from first_step 
+            have succ_cfg_correct: "(\<forall>msuc2.  List.member (out_edges(G) ! n) msuc2 \<longrightarrow> (\<forall>m3 s3. ((A,M,\<Lambda>,\<Gamma>,\<Omega>,G \<turnstile> (Inl(msuc2), inter_state) -n\<rightarrow>* (m3, s3)) \<longrightarrow> s3 \<noteq> Failure)))"
+            proof cases
+              case RedSimpleCmds show ?thesis using 2 eq RedSimpleCmds(3) dag_verifies_propagate assms(5) Rel_Main_test(1) cfg_correct by blast
+            qed (auto simp add: \<open>cs1 \<noteq> Nil\<close>)
+
+            have "j'' < j" using 1 3 using Suc_lessD by blast
+            
+            thus ?thesis using eq snd_rest_of_steps succ_correct None 2 succ_cfg_correct by blast
+          next
+            case RedParsedIfFalse
+            hence eq: "(snd_inter_bb, snd_inter_cont, snd_inter_state) = (else0, convert_list_to_cont (rev else_bbs) cont0, inter_state)" using None bb_successor_if 1 by auto
+
+            from first_step 
+            have succ_cfg_correct: "(\<forall>msuc2.  List.member (out_edges(G) ! n) msuc2 \<longrightarrow> (\<forall>m3 s3. ((A,M,\<Lambda>,\<Gamma>,\<Omega>,G \<turnstile> (Inl(msuc2), inter_state) -n\<rightarrow>* (m3, s3)) \<longrightarrow> s3 \<noteq> Failure)))"
+            proof cases
+              case RedSimpleCmds show ?thesis using 2 eq RedSimpleCmds(3) dag_verifies_propagate assms(5) Rel_Main_test(1) cfg_correct by blast
+            qed (auto simp add: \<open>cs1 \<noteq> Nil\<close>)
+
+            have "j'' < j" using 1 3 using Suc_lessD by blast
+
+            thus ?thesis using eq snd_rest_of_steps succ_correct None 2 succ_cfg_correct by blast
+          qed (auto simp add: bb_successor_if 2)
+        next
+          case (Some block_guard)
+          then show ?thesis 
+          proof cases
+            assume guard_true: "(red_expr A \<Lambda> \<Gamma> \<Omega> block_guard x1 (BoolV True))"
+            hence guard_not_false: "\<not> (red_expr A \<Lambda> \<Gamma> \<Omega> block_guard x1 (BoolV False))" using expr_eval_determ by blast
+            from snd_step have eq: "(snd_inter_bb, snd_inter_cont, snd_inter_state) = (then0, convert_list_to_cont (rev then_bbs) cont0, inter_state)" 
+            proof cases
+              case RedParsedIfTrue thus ?thesis using guard_true bb_successor_if by (simp add: RedParsedIfTrue)
+            qed (auto simp add: guard_not_false bb_successor_if 2 Some)
+
+            from first_step 
+            have succ_cfg_correct: "(\<forall>msuc2.  List.member (out_edges(G) ! n) msuc2 \<longrightarrow> (\<forall>m3 s3. ((A,M,\<Lambda>,\<Gamma>,\<Omega>,G \<turnstile> (Inl(msuc2), inter_state) -n\<rightarrow>* (m3, s3)) \<longrightarrow> s3 \<noteq> Failure)))"
+            proof cases
+              case RedSimpleCmds show ?thesis using 2 eq RedSimpleCmds(3) dag_verifies_propagate assms(5) Rel_Main_test(1) cfg_correct by blast
+            qed (auto simp add: \<open>cs1 \<noteq> Nil\<close>)
+
+            have "j'' < j" using 1 3 using Suc_lessD by blast
+            
+            thus ?thesis using eq guard_true snd_rest_of_steps succ_correct Some succ_cfg_correct 2 by blast
+          next
+            assume guard_not_true: "\<not> (red_expr A \<Lambda> \<Gamma> \<Omega> block_guard x1 (BoolV True))"
+            thus ?thesis 
+            proof cases
+              assume guard_false: "(red_expr A \<Lambda> \<Gamma> \<Omega> block_guard x1 (BoolV False))"
+              from snd_step have eq: "(snd_inter_bb, snd_inter_cont, snd_inter_state) = (else0, convert_list_to_cont (rev else_bbs) cont0, inter_state)" 
+              proof cases
+                case RedParsedIfFalse thus ?thesis using guard_false bb_successor_if by (simp add: RedParsedIfFalse)
+              qed (auto simp add: guard_not_true bb_successor_if 2 Some)
+
+              from first_step 
+              have succ_cfg_correct: "(\<forall>msuc2.  List.member (out_edges(G) ! n) msuc2 \<longrightarrow> (\<forall>m3 s3. ((A,M,\<Lambda>,\<Gamma>,\<Omega>,G \<turnstile> (Inl(msuc2), inter_state) -n\<rightarrow>* (m3, s3)) \<longrightarrow> s3 \<noteq> Failure)))"
+              proof cases
+                case RedSimpleCmds show ?thesis using 2 eq RedSimpleCmds(3) dag_verifies_propagate assms(5) Rel_Main_test(1) cfg_correct by blast
+              qed (auto simp add: \<open>cs1 \<noteq> Nil\<close>)              
+
+              have "j'' < j" using 1 3 using Suc_lessD by blast
+        
+              thus ?thesis using eq guard_false snd_rest_of_steps succ_correct Some 2 succ_cfg_correct by blast
+            next
+              assume guard_not_false2: "(\<not> (red_expr A \<Lambda> \<Gamma> \<Omega> block_guard x1 (BoolV False)))" and  
+                     guard_not_true2: "(\<not> (red_expr A \<Lambda> \<Gamma> \<Omega> block_guard x1 (BoolV True)))"
+              thus ?thesis
+              proof -
+                from snd_step have False using guard_not_false2 guard_not_true2 bb_successor_if Some 2 
+                  by (cases) auto
+                thus ?thesis by simp
+              qed
+            qed  
+          qed 
+        qed
+      qed
+    next
+      case Failure
+      then show ?thesis
+        using \<open>inter_state \<noteq> Failure \<and> (\<forall>ns1'. inter_state = Normal ns1' \<longrightarrow> A,M,\<Lambda>,\<Gamma>,\<Omega> \<turnstile> \<langle>cs2,Normal ns1\<rangle> [\<rightarrow>] Normal ns1')\<close> 
+        by linarith
+    next
+      case Magic
+      then show ?thesis by (metis Ast.valid_configuration_def a2 get_state.simps magic_propagates rest_of_steps state.distinct(3))
+    qed
+  qed
+qed auto
+
+text \<open>Global lemma for an ast-bigblock with a non-empty set of simple cmds which is the first bigblock in the else-branch of an if-statement.\<close>
+lemma block_global_rel_if_false:
+  assumes block_rel: "ast_cfg_rel None [] (BigBlock name cs1 any_str any_tr) cs2"
+  and ast_trace: "A,M,\<Lambda>,\<Gamma>,\<Omega>,T \<turnstile> ((BigBlock name cs1 any_str any_tr), cont0, (Normal ns1)) -n\<longrightarrow>^j (reached_bb, reached_cont, reached_state)"
+  and "cs1 \<noteq> Nil"
+  and "cs2 \<noteq> Nil"
+  and "node_to_block(G) ! n = cs3"
+  and "cs3 = (c#cs2)"
+  and cfg_correct: "(\<And> m2 s2. ((red_cfg_multi A M \<Lambda> \<Gamma> \<Omega> G (Inl n, Normal ns1) (m2, s2)) \<Longrightarrow> (s2 \<noteq> Failure)))"
+  and trivial_bb_successor: "(cont0 = KSeq bb1 cont1) \<and> any_str = None \<and> any_tr = None"
+  and "c = Assume some_cmd"
+  and "(UnOp Not block_guard) \<sim> some_cmd"
+  and trace_is_possible: "A,\<Lambda>,\<Gamma>,\<Omega> \<turnstile> \<langle>(UnOp Not block_guard), ns1\<rangle> \<Down> LitV (LBool True)"
+  and block_local_rel: 
+        "\<And> reached_bb_inter reached_cont_inter reached_state_inter. (red_bigblock A M \<Lambda> \<Gamma> \<Omega> T ((BigBlock name cs1 any_str any_tr), cont0, (Normal ns1)) (reached_bb_inter, reached_cont_inter, reached_state_inter)) \<Longrightarrow> 
+        (\<And> s2'.((red_cmd_list A M \<Lambda> \<Gamma> \<Omega> cs3 (Normal ns1) s2') \<Longrightarrow> (s2' \<noteq> Failure))) \<Longrightarrow>   
+        (reached_state_inter \<noteq> Failure  \<and> (\<forall>ns1'. reached_state_inter = Normal ns1' \<longrightarrow> (A,M,\<Lambda>,\<Gamma>,\<Omega> \<turnstile> \<langle>cs3, Normal ns1\<rangle> [\<rightarrow>] Normal ns1')))"
+  and succ_correct: 
+       "\<And>  ns1'' k.
+        k < j \<Longrightarrow> 
+        \<forall>msuc2.  List.member (out_edges(G) ! n) msuc2 \<longrightarrow> (\<forall>m3 s3. ((A,M,\<Lambda>,\<Gamma>,\<Omega>,G \<turnstile> (Inl(msuc2), Normal ns1'') -n\<rightarrow>* (m3, s3)) \<longrightarrow> s3 \<noteq> Failure)) \<Longrightarrow>
+        A,M,\<Lambda>,\<Gamma>,\<Omega>,T \<turnstile> (bb1, cont1, (Normal ns1'')) -n\<longrightarrow>^k (reached_bb, reached_cont, reached_state) \<Longrightarrow> 
+        (Ast.valid_configuration A \<Lambda> \<Gamma> \<Omega> posts reached_bb reached_cont reached_state)"
+     shows "(Ast.valid_configuration A \<Lambda> \<Gamma> \<Omega> posts reached_bb reached_cont reached_state)" 
+  using assms
+proof cases
+  case Rel_Main_test
+  have not_end: "(cont0 \<noteq> KStop) \<or> any_str \<noteq> None \<or> any_tr \<noteq> None" using trivial_bb_successor by simp
+  from ast_trace show ?thesis
+  proof (cases j)
+    case 0
+    hence "(reached_bb, reached_cont, reached_state) = ((BigBlock name cs1 any_str any_tr), cont0, (Normal ns1))" using ast_trace by fastforce
+    then show ?thesis unfolding Ast.valid_configuration_def by (simp add: trivial_bb_successor)
+  next
+    case succ_0: (Suc j')
+    from this obtain inter_bb inter_cont inter_state where
+      first_step: "red_bigblock A M \<Lambda> \<Gamma> \<Omega> T ((BigBlock name cs1 any_str any_tr), cont0, (Normal ns1)) (inter_bb, inter_cont, inter_state)" and
+      rest_of_steps: "A,M,\<Lambda>,\<Gamma>,\<Omega>,T \<turnstile> (inter_bb, inter_cont, inter_state) -n\<longrightarrow>^j' (reached_bb, reached_cont, reached_state)" 
+      by (metis ast_trace prod_cases3 relpowp_Suc_D2)
+
+    from cfg_correct \<open>cs2 \<noteq> Nil\<close> \<open>node_to_block(G) ! n = cs3\<close> 
+    have local_rel_corr: "(\<And> s2'.((red_cmd_list A M \<Lambda> \<Gamma> \<Omega> cs3 (Normal ns1) s2') \<Longrightarrow> (s2' \<noteq> Failure)))"
+      using dag_verifies_propagate_2 by blast
+
+    from local_rel_corr first_step 
+    have a2: "(inter_state \<noteq> Failure  \<and> (\<forall>ns1'. inter_state = Normal ns1' \<longrightarrow> (A,M,\<Lambda>,\<Gamma>,\<Omega> \<turnstile> \<langle>cs3, Normal ns1\<rangle> [\<rightarrow>] Normal ns1')))" 
+      using block_local_rel by simp
+
+    from first_step \<open>cs1 \<noteq> Nil\<close> 
+    have a1: "(inter_bb, inter_cont, inter_state) = ((BigBlock name [] any_str any_tr), cont0, inter_state)"
+    proof cases
+      case RedSimpleCmds then show ?thesis by (auto simp add: RedSimpleCmds)
+    qed auto
+
+    show ?thesis 
+    proof (cases inter_state)
+      case 1: (Normal x1)
+      from rest_of_steps show ?thesis 
+      proof (cases j')
+        case 0
+        then show ?thesis
+          by (metis Ast.valid_configuration_def a1 a2 get_state.simps is_final.simps(5) relpowp_0_E rest_of_steps trivial_bb_successor)
+      next
+        case 2: (Suc j'')
+        from this rest_of_steps obtain snd_inter_bb snd_inter_cont snd_inter_state where
+          snd_step: "red_bigblock A M \<Lambda> \<Gamma> \<Omega> T ((BigBlock name [] any_str any_tr), cont0, inter_state)  (snd_inter_bb, snd_inter_cont, snd_inter_state)" and
+          snd_rest_of_steps: "A,M,\<Lambda>,\<Gamma>,\<Omega>,T \<turnstile> (snd_inter_bb, snd_inter_cont, snd_inter_state) -n\<longrightarrow>^j'' (reached_bb, reached_cont, reached_state)"
+          by (metis a1 get_state.cases relpowp_Suc_D2)
+        from snd_step have snd_step_equiv: "(snd_inter_bb, snd_inter_cont, snd_inter_state) = (bb1, cont1, inter_state)"
+        proof cases
+          case RedSkip thus ?thesis using trivial_bb_successor by (simp add: RedSkip)
+        qed (auto simp add: trivial_bb_successor "1")
+
+        from first_step 
+        have succ_cfg_correct: "(\<forall>msuc2.  List.member (out_edges(G) ! n) msuc2 \<longrightarrow> (\<forall>m3 s3. ((A,M,\<Lambda>,\<Gamma>,\<Omega>,G \<turnstile> (Inl(msuc2), inter_state) -n\<rightarrow>* (m3, s3)) \<longrightarrow> s3 \<noteq> Failure)))"
+        proof cases
+          case RedSimpleCmds 
+          hence cmds_red: "A,M,\<Lambda>,\<Gamma>,\<Omega> \<turnstile> \<langle>c#cs2, Normal ns1\<rangle> [\<rightarrow>] inter_state" 
+            using Rel_Main_test(1) \<open>c = Assume some_cmd\<close> \<open>(UnOp Not block_guard) \<sim> some_cmd\<close> equiv_preserves_value trace_is_possible RedAssumeOk RedCmdListCons 
+            by metis
+          show ?thesis by (metis (no_types, lifting) "1" RedNormalSucc assms(5) assms(6) cfg_correct cmds_red converse_rtranclp_into_rtranclp)
+        qed (auto simp add: \<open>cs1 \<noteq> Nil\<close>) 
+
+        have "j'' < j" using succ_0 2 by simp
+
+        then show ?thesis using snd_step_equiv succ_correct snd_rest_of_steps "1" succ_cfg_correct by blast 
+      qed
+    next
+      case Failure
+      then show ?thesis
+        using \<open>inter_state \<noteq> Failure \<and> (\<forall>ns1'. inter_state = Normal ns1' \<longrightarrow> A,M,\<Lambda>,\<Gamma>,\<Omega> \<turnstile> \<langle>cs3,Normal ns1\<rangle> [\<rightarrow>] Normal ns1')\<close> 
+        by linarith
+    next
+      case Magic
+      then show ?thesis by (metis Ast.valid_configuration_def a2 get_state.simps magic_propagates rest_of_steps state.distinct(3))
+    qed
+  qed
+qed auto
+
+text \<open>Global lemma for an ast-bigblock with a non-empty set of simple cmds which is the first bigblock in the then-branch of an if-statement.\<close>
+lemma block_global_rel_if_true:
+  assumes block_rel: "ast_cfg_rel None [] (BigBlock name cs1 any_str any_tr) cs2"
+  and ast_trace: "A,M,\<Lambda>,\<Gamma>,\<Omega>,T \<turnstile> ((BigBlock name cs1 any_str any_tr), cont0, (Normal ns1)) -n\<longrightarrow>^j (reached_bb, reached_cont, reached_state)"
+  and "cs1 \<noteq> Nil"
+  and "cs2 \<noteq> Nil"
+  and "node_to_block(G) ! n = cs3"
+  and "cs3 = c#cs2"
+  and cfg_correct: "(\<And> m2 s2. ((red_cfg_multi A M \<Lambda> \<Gamma> \<Omega> G (Inl n, Normal ns1) (m2, s2)) \<Longrightarrow> (s2 \<noteq> Failure)))"
+  and trivial_bb_successor: "(cont0 = KSeq bb1 cont1) \<and> any_str = None \<and> any_tr = None"
+  and "c = Assume block_guard"
+  and trace_is_possible: "A,\<Lambda>,\<Gamma>,\<Omega> \<turnstile> \<langle>block_guard, ns1\<rangle> \<Down> LitV (LBool True)"
+  and block_local_rel: 
+        "\<And> reached_bb_inter reached_cont_inter reached_state_inter. (red_bigblock A M \<Lambda> \<Gamma> \<Omega> T ((BigBlock name cs1 any_str any_tr), cont0, (Normal ns1)) (reached_bb_inter, reached_cont_inter, reached_state_inter)) \<Longrightarrow> 
+        (\<And> s2'.((red_cmd_list A M \<Lambda> \<Gamma> \<Omega> cs3 (Normal ns1) s2') \<Longrightarrow> (s2' \<noteq> Failure))) \<Longrightarrow>   
+        (reached_state_inter \<noteq> Failure  \<and> (\<forall>ns1'. reached_state_inter = Normal ns1' \<longrightarrow> (A,M,\<Lambda>,\<Gamma>,\<Omega> \<turnstile> \<langle>cs3, Normal ns1\<rangle> [\<rightarrow>] Normal ns1')))"
+  and succ_correct: 
+       "\<And>  ns1'' k.
+        k < j \<Longrightarrow> 
+        \<forall>msuc2.  List.member (out_edges(G) ! n) msuc2 \<longrightarrow> (\<forall>m3 s3. ((A,M,\<Lambda>,\<Gamma>,\<Omega>,G \<turnstile> (Inl(msuc2), Normal ns1'') -n\<rightarrow>* (m3, s3)) \<longrightarrow> s3 \<noteq> Failure)) \<Longrightarrow>
+        A,M,\<Lambda>,\<Gamma>,\<Omega>,T \<turnstile> (bb1, cont1, (Normal ns1'')) -n\<longrightarrow>^k (reached_bb, reached_cont, reached_state) \<Longrightarrow> 
+        (Ast.valid_configuration A \<Lambda> \<Gamma> \<Omega> posts reached_bb reached_cont reached_state)"
+     shows "(Ast.valid_configuration A \<Lambda> \<Gamma> \<Omega> posts reached_bb reached_cont reached_state)" 
+  using assms
+proof cases
+  case Rel_Main_test
+  have not_end: "(cont0 \<noteq> KStop) \<or> any_str \<noteq> None \<or> any_tr \<noteq> None" using trivial_bb_successor by simp
+  from ast_trace show ?thesis
+  proof (cases j)
+    case 0
+    hence "(reached_bb, reached_cont, reached_state) = ((BigBlock name cs1 any_str any_tr), cont0, (Normal ns1))" using ast_trace by auto
+    then show ?thesis unfolding Ast.valid_configuration_def by (metis assms(3) get_state.simps is_final.simps(2) neq_Nil_conv state.distinct(1))
+  next
+    case succ_0: (Suc j')
+    from this obtain inter_bb inter_cont inter_state where
+      first_step: "red_bigblock A M \<Lambda> \<Gamma> \<Omega> T ((BigBlock name cs1 any_str any_tr), cont0, (Normal ns1)) (inter_bb, inter_cont, inter_state)" and
+      rest_of_steps: "A,M,\<Lambda>,\<Gamma>,\<Omega>,T \<turnstile> (inter_bb, inter_cont, inter_state) -n\<longrightarrow>^j' (reached_bb, reached_cont, reached_state)" 
+      by (metis ast_trace get_state.cases relpowp_Suc_D2)
+
+    from cfg_correct \<open>cs2 \<noteq> Nil\<close> \<open>node_to_block(G) ! n = cs3\<close> 
+    have local_rel_corr: "(\<And> s2'.((red_cmd_list A M \<Lambda> \<Gamma> \<Omega> cs3 (Normal ns1) s2') \<Longrightarrow> (s2' \<noteq> Failure)))"
+      using dag_verifies_propagate_2 by blast
+
+    from local_rel_corr first_step 
+    have a2: "(inter_state \<noteq> Failure  \<and> (\<forall>ns1'. inter_state = Normal ns1' \<longrightarrow> (A,M,\<Lambda>,\<Gamma>,\<Omega> \<turnstile> \<langle>cs3, Normal ns1\<rangle> [\<rightarrow>] Normal ns1')))" 
+      using block_local_rel by simp
+
+    from first_step \<open>cs1 \<noteq> Nil\<close> 
+    have a1: "(inter_bb, inter_cont, inter_state) = ((BigBlock name [] any_str any_tr), cont0, inter_state)"
+    proof cases
+      case RedSimpleCmds then show ?thesis by (auto simp add: RedSimpleCmds)
+    qed auto
+
+    show ?thesis 
+    proof (cases inter_state)
+      case 1: (Normal x1)
+      from rest_of_steps show ?thesis 
+      proof (cases j')
+        case 0
+        then show ?thesis 
+          by (metis valid_configuration_def a1 a2 get_state.simps is_final.simps(5) relpowp_0_E rest_of_steps trivial_bb_successor)
+      next
+        case 2: (Suc j'')
+        from this rest_of_steps obtain snd_inter_bb snd_inter_cont snd_inter_state where
+          snd_step: "red_bigblock A M \<Lambda> \<Gamma> \<Omega> T ((BigBlock name [] any_str any_tr), cont0, inter_state)  (snd_inter_bb, snd_inter_cont, snd_inter_state)" and
+          snd_rest_of_steps: "A,M,\<Lambda>,\<Gamma>,\<Omega>,T \<turnstile> (snd_inter_bb, snd_inter_cont, snd_inter_state) -n\<longrightarrow>^j'' (reached_bb, reached_cont, reached_state)"
+          by (metis a1 get_state.cases relpowp_Suc_D2)
+
+        from snd_step have snd_step_equiv: "(snd_inter_bb, snd_inter_cont, snd_inter_state) = (bb1, cont1, inter_state)"
+        proof cases
+          case RedSkip thus ?thesis using trivial_bb_successor by (simp add: RedSkip)
+        qed (auto simp add: trivial_bb_successor "1")
+
+        from first_step 
+        have succ_cfg_correct: "(\<forall>msuc2.  List.member (out_edges(G) ! n) msuc2 \<longrightarrow> (\<forall>m3 s3. ((A,M,\<Lambda>,\<Gamma>,\<Omega>,G \<turnstile> (Inl(msuc2), inter_state) -n\<rightarrow>* (m3, s3)) \<longrightarrow> s3 \<noteq> Failure)))"
+        proof cases
+          case RedSimpleCmds 
+          hence cmds_red: "A,M,\<Lambda>,\<Gamma>,\<Omega> \<turnstile> \<langle>c#cs2, Normal ns1\<rangle> [\<rightarrow>] inter_state" 
+            using Rel_Main_test(1) \<open>c = Assume block_guard\<close> trace_is_possible RedAssumeOk RedCmdListCons by blast
+          show ?thesis using "1" assms(5) assms(6) cfg_correct cmds_red dag_verifies_propagate by blast
+        qed (auto simp add: \<open>cs1 \<noteq> Nil\<close>) 
+
+        have "j'' < j" using succ_0 2 by simp
+
+        then show ?thesis using snd_step_equiv succ_correct snd_rest_of_steps "1" succ_cfg_correct by blast 
+      qed
+    next
+      case Failure
+      then show ?thesis
+        using \<open>inter_state \<noteq> Failure \<and> (\<forall>ns1'. inter_state = Normal ns1' \<longrightarrow> A,M,\<Lambda>,\<Gamma>,\<Omega> \<turnstile> \<langle>cs3,Normal ns1\<rangle> [\<rightarrow>] Normal ns1')\<close> 
+        by linarith
+    next
+      case Magic
+      then show ?thesis by (metis valid_configuration_def a2 get_state.simps magic_propagates rest_of_steps state.simps(5))
+    qed
+  qed
+qed auto
+
+text \<open>Global lemma for a generic ast-bigblock with a non-empty set of simple cmds.\<close>
+lemma block_global_rel_generic:
+  assumes block_rel: "ast_cfg_rel None [] (BigBlock name cs1 any_str any_tr) cs2"
+  and ast_trace: "A,M,\<Lambda>,\<Gamma>,\<Omega>,T \<turnstile> ((BigBlock name cs1 any_str any_tr), cont0, (Normal ns1)) -n\<longrightarrow>^j (reached_bb, reached_cont, reached_state)"
+  and "cs1 \<noteq> Nil"
+  and "cs2 \<noteq> Nil"
+  and "node_to_block(G) ! n = cs2"
+  and cfg_correct: "(\<And> m2 s2. ((red_cfg_multi A M \<Lambda> \<Gamma> \<Omega> G (Inl n, Normal ns1) (m2, s2)) \<Longrightarrow> (s2 \<noteq> Failure)))"
+  and trivial_bb_successor: "(cont0 = KSeq bb1 cont1) \<and> any_str = None \<and> any_tr = None"
+  and block_local_rel: 
+        "\<And> reached_bb_inter reached_cont_inter reached_state_inter. (red_bigblock A M \<Lambda> \<Gamma> \<Omega> T ((BigBlock name cs1 any_str any_tr), cont0, (Normal ns1)) (reached_bb_inter, reached_cont_inter, reached_state_inter)) \<Longrightarrow> 
+        (\<And> s2'.((red_cmd_list A M \<Lambda> \<Gamma> \<Omega> cs2 (Normal ns1) s2') \<Longrightarrow> (s2' \<noteq> Failure))) \<Longrightarrow>   
+        (reached_state_inter \<noteq> Failure  \<and> (\<forall>ns1'. reached_state_inter = Normal ns1' \<longrightarrow> (A,M,\<Lambda>,\<Gamma>,\<Omega> \<turnstile> \<langle>cs2, Normal ns1\<rangle> [\<rightarrow>] Normal ns1')))"
+  and succ_correct: 
+       "\<And>  ns1'' k.
+        k < j \<Longrightarrow> 
+        \<forall>msuc2.  List.member (out_edges(G) ! n) msuc2 \<longrightarrow> (\<forall>m3 s3. ((A,M,\<Lambda>,\<Gamma>,\<Omega>,G \<turnstile> (Inl(msuc2), Normal ns1'') -n\<rightarrow>* (m3, s3)) \<longrightarrow> s3 \<noteq> Failure)) \<Longrightarrow>
+        A,M,\<Lambda>,\<Gamma>,\<Omega>,T \<turnstile> (bb1, cont1, (Normal ns1'')) -n\<longrightarrow>^k (reached_bb, reached_cont, reached_state) \<Longrightarrow> 
+        (Ast.valid_configuration A \<Lambda> \<Gamma> \<Omega> posts reached_bb reached_cont reached_state)"
+  shows "(Ast.valid_configuration A \<Lambda> \<Gamma> \<Omega> posts reached_bb reached_cont reached_state)" 
+  using assms
+proof cases
+  case Rel_Main_test
+  have not_end: "(cont0 \<noteq> KStop) \<or> any_str \<noteq> None \<or> any_tr \<noteq> None" using trivial_bb_successor by simp
+  from ast_trace show ?thesis
+  proof (cases j)
+    case 0
+    hence "(reached_bb, reached_cont, reached_state) = ((BigBlock name cs1 any_str any_tr), cont0, (Normal ns1))" using ast_trace by auto
+    then show ?thesis unfolding Ast.valid_configuration_def by (simp add: trivial_bb_successor)
+  next
+    case succ_0: (Suc j')
+    from this obtain inter_bb inter_cont inter_state where
+      first_step: "red_bigblock A M \<Lambda> \<Gamma> \<Omega> T ((BigBlock name cs1 any_str any_tr), cont0, (Normal ns1)) (inter_bb, inter_cont, inter_state)" and
+      rest_of_steps: "A,M,\<Lambda>,\<Gamma>,\<Omega>,T \<turnstile> (inter_bb, inter_cont, inter_state) -n\<longrightarrow>^j' (reached_bb, reached_cont, reached_state)"
+      by (metis ast_trace get_state.cases relpowp_Suc_D2)
+
+    from cfg_correct \<open>cs2 \<noteq> Nil\<close> \<open>node_to_block(G) ! n = cs2\<close> 
+    have local_rel_corr: "(\<And> s2'.((red_cmd_list A M \<Lambda> \<Gamma> \<Omega> cs2 (Normal ns1) s2') \<Longrightarrow> (s2' \<noteq> Failure)))"
+      using dag_verifies_propagate_2 by blast
+
+    from local_rel_corr first_step 
+    have a2: "(inter_state \<noteq> Failure  \<and> (\<forall>ns1'. inter_state = Normal ns1' \<longrightarrow> (A,M,\<Lambda>,\<Gamma>,\<Omega> \<turnstile> \<langle>cs2, Normal ns1\<rangle> [\<rightarrow>] Normal ns1')))" 
+      using block_local_rel by simp
+
+    from first_step \<open>cs1 \<noteq> Nil\<close> 
+    have a1: "(inter_bb, inter_cont, inter_state) = ((BigBlock name [] any_str any_tr), cont0, inter_state)"
+    proof cases
+      case RedSimpleCmds then show ?thesis by (auto simp add: RedSimpleCmds)
+    qed auto
+
+    show ?thesis 
+    proof (cases inter_state)
+      case 1: (Normal x1)
+      from rest_of_steps show ?thesis 
+      proof (cases j')
+        case 0
+        then show ?thesis 
+          by (metis valid_configuration_def a1 a2 get_state.simps is_final.simps(5) relpowp_0_E rest_of_steps trivial_bb_successor)
+      next
+        case 2: (Suc j'')
+        from this rest_of_steps obtain snd_inter_bb snd_inter_cont snd_inter_state where
+          snd_step: "red_bigblock A M \<Lambda> \<Gamma> \<Omega> T ((BigBlock name [] any_str any_tr), cont0, inter_state)  (snd_inter_bb, snd_inter_cont, snd_inter_state)" and
+          snd_rest_of_steps: "A,M,\<Lambda>,\<Gamma>,\<Omega>,T \<turnstile> (snd_inter_bb, snd_inter_cont, snd_inter_state) -n\<longrightarrow>^j'' (reached_bb, reached_cont, reached_state)"
+          by (metis a1 get_state.cases relpowp_Suc_D2)
+
+        from snd_step have snd_step_equiv: "(snd_inter_bb, snd_inter_cont, snd_inter_state) = (bb1, cont1, inter_state)"
+        proof cases
+          case RedSkip thus ?thesis using trivial_bb_successor by (simp add: RedSkip)
+        qed (auto simp add: trivial_bb_successor "1")
+
+        from first_step 
+        have succ_cfg_correct: "(\<forall>msuc2.  List.member (out_edges(G) ! n) msuc2 \<longrightarrow> (\<forall>m3 s3. ((A,M,\<Lambda>,\<Gamma>,\<Omega>,G \<turnstile> (Inl(msuc2), inter_state) -n\<rightarrow>* (m3, s3)) \<longrightarrow> s3 \<noteq> Failure)))"
+        proof cases
+          case RedSimpleCmds show ?thesis using 1 snd_step_equiv  RedSimpleCmds(3) dag_verifies_propagate Rel_Main_test(1) cfg_correct assms(5) by blast
+        qed (auto simp add: \<open>cs1 \<noteq> Nil\<close>) 
+
+        have "j'' < j" using succ_0 2 by simp
+
+        then show ?thesis using snd_step_equiv succ_correct snd_rest_of_steps "1" succ_cfg_correct by blast
+      qed
+    next
+      case Failure
+      then show ?thesis
+        using \<open>inter_state \<noteq> Failure \<and> (\<forall>ns1'. inter_state = Normal ns1' \<longrightarrow> A,M,\<Lambda>,\<Gamma>,\<Omega> \<turnstile> \<langle>cs2,Normal ns1\<rangle> [\<rightarrow>] Normal ns1')\<close> 
+        by linarith
+    next
+      case Magic
+      then show ?thesis by (metis valid_configuration_def a2 get_state.simps magic_propagates rest_of_steps state.distinct(3))
+    qed
+  qed
+qed auto
+
+text \<open>Helper lemmas used to complete the procedure correctness proof\<close>
+
+lemma end_to_end_util2:
+  assumes AExpanded: "\<And> \<Gamma> end_bb end_cont end_state ns M.
+           rtranclp (red_bigblock B M \<Lambda> \<Gamma> [] ast) (init_ast ast ns) (end_bb, end_cont, end_state) \<Longrightarrow>
+           (\<And> v. (closed ((type_of_val B) v))) \<Longrightarrow>
+           (\<And> t. ((closed t) \<Longrightarrow> (\<exists> v. (((type_of_val B) v) = t)))) \<Longrightarrow>
+           (fun_interp_wf B fun_decls \<Gamma>) \<Longrightarrow>
+           (axiom_assm B \<Gamma> constants (ns::(('a)nstate)) axioms) \<Longrightarrow>
+           (expr_all_sat B \<Lambda> \<Gamma> [] ns all_pres) \<Longrightarrow>
+           (state_typ_wf B [] (local_state ns) (snd \<Lambda>)) \<Longrightarrow>
+           (state_typ_wf B [] (global_state ns) (fst \<Lambda>)) \<Longrightarrow>
+           ((global_state ns) = (old_global_state ns)) \<Longrightarrow>
+           ((binder_state ns) = Map.empty) \<Longrightarrow> 
+           (Ast.valid_configuration B \<Lambda> \<Gamma> [] checked_posts end_bb end_cont end_state)" and
+          "all_pres = proc_all_pres proc_ast" and
+          "checked_posts = proc_checked_posts proc_ast" and
+          ABody: "ast_procedure.proc_body proc_ast = Some (locals, ast)" and
+          AVarContext:"\<Lambda> = (constants@global_vars, (proc_args proc_ast)@locals)" and
+          ARets:"proc_rets proc_ast = []" and
+         (* "fun_decls = prog_funcs prog" and
+          "axs = prog_axioms prog" and*)
+          "proc_ty_args proc_ast = 0" 
+          (*"const_decls = prog_consts prog"*)
+  shows "Ast.proc_is_correct B fun_decls constants global_vars axioms proc_ast"
+proof -
+  show "proc_is_correct B fun_decls constants global_vars axioms proc_ast"
+  proof( (simp only: proc_is_correct.simps), subst ABody, simp split: option.split, (rule allI | rule impI)+,
+         unfold proc_body_satisfies_spec_def,(rule allI | rule impI)+)  
+    fix \<Gamma> \<Omega> gs ls end_bb end_cont end_state
+    assume Atyp:"(\<forall>t. closed t \<longrightarrow> (\<exists>v. type_of_val B v = t)) \<and> (\<forall>v. closed (type_of_val B v))" and
+           FunWf:"fun_interp_wf B fun_decls \<Gamma>" and
+           ARenv: "list_all closed \<Omega> \<and> length \<Omega> = proc_ty_args proc_ast" and
+           WfGlobal: "state_typ_wf B \<Omega> gs (constants @ global_vars)" and
+           WfLocal: "state_typ_wf B \<Omega> ls (proc_args proc_ast @ locals @ proc_rets proc_ast)" and
+           AxSat: "axioms_sat B (constants, []) \<Gamma>
+        \<lparr>old_global_state = Map.empty, global_state = state_restriction gs constants, local_state = Map.empty, binder_state = Map.empty\<rparr>
+        axioms" and
+        APres:  "expr_all_sat B (constants @ global_vars, proc_args proc_ast @ locals @ proc_rets proc_ast) \<Gamma> \<Omega>
+        \<lparr>old_global_state = gs, global_state = gs, local_state = ls, binder_state = Map.empty\<rparr> (map fst (proc_pres proc_ast))" and
+        Ared: "rtranclp 
+               (red_bigblock 
+                B [] (constants @ global_vars,
+                proc_args proc_ast @
+                locals @
+                proc_rets
+                 proc_ast) \<Gamma> \<Omega> ast) (init_ast ast \<lparr>old_global_state = gs, global_state = gs, local_state = ls, binder_state = Map.empty\<rparr>)
+       (end_bb, end_cont, end_state)"
+    have Contexteq:"\<Lambda> = (constants @ global_vars, proc_args proc_ast @ locals @ proc_rets proc_ast)"
+      using AVarContext ARets by simp
+    from ARenv \<open>proc_ty_args proc_ast = 0\<close> have "\<Omega> = []" by simp
+    have "Ast.valid_configuration B \<Lambda> \<Gamma> [] checked_posts end_bb end_cont end_state"
+      apply (rule AExpanded)
+                apply (subst Contexteq)
+      using Ared \<open>\<Omega> = []\<close>
+                apply fastforce
+              apply (simp add: Atyp)
+             apply (simp add: Atyp)
+            apply (simp add: FunWf)
+      unfolding nstate_global_restriction_def 
+      using AxSat
+           apply simp
+      using APres \<open>\<Omega> = []\<close> \<open>all_pres = _\<close> Contexteq
+          apply simp
+      using Contexteq WfLocal \<open>\<Omega> = []\<close>
+         apply simp
+      using Contexteq WfGlobal \<open>\<Omega> = []\<close>      
+        apply simp
+       apply simp
+      apply simp
+      done
+    thus "Ast.valid_configuration B (constants @ global_vars, proc_args proc_ast @ locals @ proc_rets proc_ast) \<Gamma> \<Omega>
+        (map fst (filter (\<lambda>x. \<not> snd x) (proc_posts proc_ast))) end_bb end_cont end_state"
+      using Contexteq \<open>\<Omega> = []\<close> \<open>checked_posts = _\<close>
+      by simp
+  qed
+qed
+
+lemma valid_config_implies_not_failure:
+  assumes "Semantics.valid_configuration A \<Lambda> \<Gamma> \<Omega> posts m' s'"
+  shows "s' \<noteq> Failure"
+  using Semantics.valid_configuration_def assms by blast
+
+end
