BoogieLang/completed_example_proofs/if_example_proofs/global_data.thy
@@ -1,0 +1,34 @@
+theory global_data
+  imports "/home/alex/boogie_related/foundational_boogie/BoogieLang/Semantics" 
+          "/home/alex/boogie_related/foundational_boogie/BoogieLang/TypeSafety" 
+          "/home/alex/boogie_related/foundational_boogie/BoogieLang/Util" 
+begin
+definition axioms
+  where
+    "axioms  = []"
+definition fdecls
+  where
+    "fdecls  = []"
+definition globals_vdecls :: "(vdecls)"
+  where
+    "globals_vdecls  = []"
+definition constants_vdecls :: "(vdecls)"
+  where
+    "constants_vdecls  = []"
+lemma globals_max_aux:
+shows "(((map fst (append global_data.constants_vdecls global_data.globals_vdecls)) \<noteq> []) \<longrightarrow> ((Max (set (map fst (append global_data.constants_vdecls global_data.globals_vdecls)))) \<le> 0))"
+unfolding global_data.constants_vdecls_def global_data.globals_vdecls_def
+by simp
+
+lemma globals_max:
+shows "(\<forall> x. ((Set.member x (set (map fst (append global_data.constants_vdecls global_data.globals_vdecls)))) \<longrightarrow> (x \<le> 0)))"
+using globals_max_aux helper_max
+by blast
+
+lemma funcs_wf:
+shows "((list_all (comp wf_fdecl snd) fdecls) )"
+unfolding fdecls_def
+by simp
+
+
+end
