BoogieLang/completed_example_proofs/if_example_proofs/p_proofs/if_example_ast_cfg_proof.thy
@@ -1,0 +1,295 @@
+theory if_example_ast_cfg_proof
+  imports Main
+          Boogie_Lang.Ast
+          Boogie_Lang.Semantics
+          Boogie_Lang.Ast_Cfg_Transformation
+          "../global_data" 
+          p_before_cfg_to_dag_prog 
+          if_example_before_ast_cfg
+          p_cfgtodag_proof
+          "/home/alex/Isabelle_10-Nov-2021/lib/Apply_Trace_Cmd"
+          p_before_passive_prog 
+          p_passification_proof 
+          p_vcphase_proof
+
+begin
+
+abbreviation bigblock_then 
+  where "bigblock_then \<equiv> BigBlock None [(Assign 0 (Lit (LInt 10)))] None None"
+
+abbreviation bigblock_else
+  where "bigblock_else \<equiv> BigBlock None [(Assign 0 (Lit (LInt 1)))] None None"
+
+lemma bigblock0_local_rel:
+  assumes Red_bb0_to: 
+      "red_bigblock A M \<Lambda> \<Gamma> \<Omega> T (bigblock0, KSeq bigblock1 KStop, (Normal ns1)) (reached_bb, reached_cont, reached_state)" 
+  and Red0_impl: "(\<And> s2'.(red_cmd_list A M \<Lambda> \<Gamma> \<Omega> [Havoc 0] (Normal ns1) s2') \<Longrightarrow> s2' \<noteq> Failure)" 
+  shows "reached_state \<noteq> Failure \<and> 
+         (\<forall>ns1'. reached_state = Normal ns1' \<longrightarrow> (A,M,\<Lambda>,\<Gamma>,\<Omega> \<turnstile> \<langle>[Havoc 0], Normal ns1\<rangle> [\<rightarrow>] Normal ns1'))"
+proof -
+  have "ast_cfg_rel None [] bigblock0 p_before_cfg_to_dag_prog.block_0" 
+    unfolding p_before_cfg_to_dag_prog.block_0_def
+    by (rule Rel_Main_test)
+  then show ?thesis 
+    using assms
+    unfolding p_before_cfg_to_dag_prog.block_0_def
+    by (auto simp: block_local_rel_generic) 
+qed
+
+
+lemma bigblock_then_local_rel:
+  assumes Red_bb0_to: "red_bigblock A M \<Lambda> \<Gamma> \<Omega> T (bigblock_then, KSeq bigblock1 KStop, (Normal ns1)) (reached_bb, reached_cont, reached_state)" 
+  and Red0_impl: "(\<And> s2'.(red_cmd_list A M \<Lambda> \<Gamma> \<Omega> p_before_cfg_to_dag_prog.block_3 (Normal ns1) s2') \<Longrightarrow> s2' \<noteq> Failure)" 
+  and trace_is_possible: "A,\<Lambda>,\<Gamma>,\<Omega> \<turnstile> \<langle>(BinOp (Var 0) Gt (Lit (LInt 5))), ns1\<rangle> \<Down> LitV (LBool True)"
+  shows "reached_state \<noteq> Failure \<and> 
+         (\<forall>ns1'. reached_state = Normal ns1' \<longrightarrow> (A,M,\<Lambda>,\<Gamma>,\<Omega> \<turnstile> \<langle>p_before_cfg_to_dag_prog.block_3, Normal ns1\<rangle> [\<rightarrow>] Normal ns1'))" 
+proof -
+  have syntactic_rel: "ast_cfg_rel None [] bigblock_then [(Assign 0 (Lit (LInt 10)))]" 
+    by (rule Rel_Main_test)
+  show ?thesis
+    unfolding p_before_cfg_to_dag_prog.block_3_def 
+    apply (rule block_local_rel_guard_true[OF syntactic_rel _ _ _  trace_is_possible Red_bb0_to Red0_impl])
+    unfolding p_before_cfg_to_dag_prog.block_3_def 
+    by simp_all
+qed
+
+lemma bigblock_else_local_rel:
+  assumes Red_bb0_to: "red_bigblock A M \<Lambda> \<Gamma> \<Omega> T (bigblock_else, KSeq bigblock1 KStop, (Normal ns1)) (reached_bb, reached_cont, reached_state)" 
+  and Red0_impl: "(\<And> s2'.(red_cmd_list A M \<Lambda> \<Gamma> \<Omega> p_before_cfg_to_dag_prog.block_1 (Normal ns1) s2') \<Longrightarrow> s2' \<noteq> Failure)" 
+  and trace_is_possible: "A,\<Lambda>,\<Gamma>,\<Omega> \<turnstile> \<langle>UnOp Not (BinOp (Var 0) Gt (Lit (LInt 5))), ns1\<rangle> \<Down> LitV (LBool True)"
+  shows "reached_state \<noteq> Failure \<and> 
+         (\<forall>ns1'. reached_state = Normal ns1' \<longrightarrow> (A,M,\<Lambda>,\<Gamma>,\<Omega> \<turnstile> \<langle>p_before_cfg_to_dag_prog.block_1, Normal ns1\<rangle> [\<rightarrow>] Normal ns1'))"
+proof -
+  have syntactic_rel: "ast_cfg_rel None [] bigblock_else [(Assign 0 (Lit (LInt 1)))]"
+    by (rule Rel_Main_test)
+  have guard_equiv: "UnOp Not (BinOp (Var 0) Gt (Lit (LInt 5))) \<sim> (Lit (LInt 5) \<guillemotleft>Ge\<guillemotright> Var 0)" 
+    by (rule neg_gt2)
+  show ?thesis
+    unfolding p_before_cfg_to_dag_prog.block_1_def 
+    apply (rule block_local_rel_guard_false[OF syntactic_rel _ _ guard_equiv _ trace_is_possible Red_bb0_to Red0_impl])
+    unfolding p_before_cfg_to_dag_prog.block_1_def
+    by simp_all
+qed
+
+lemma block2_global_rel:
+  assumes concrete_trace: "A,M,\<Lambda>,\<Gamma>,\<Omega>,T \<turnstile> (bigblock1, KStop, (Normal ns1)) -n\<longrightarrow>^j (reached_bb, reached_cont, reached_state)"
+  and cfg_is_correct: "\<And> m' s'. (red_cfg_multi A M \<Lambda> \<Gamma> \<Omega> p_before_cfg_to_dag_prog.proc_body ((Inl 2),(Normal ns1)) (m',s')) \<Longrightarrow> (s' \<noteq> Failure)" 
+  shows "(Ast.valid_configuration A \<Lambda> \<Gamma> \<Omega> [] reached_bb reached_cont reached_state)" 
+  using assms
+proof -
+  have syn_rel: "ast_cfg_rel None [] bigblock1 [(Assert (BinOp (Var 0) Gt (Lit (LInt 0))))]" using Rel_Main_test by blast 
+  have cmds: "node_to_block p_before_cfg_to_dag_prog.proc_body ! 2 = [(Assert (BinOp (Var 0) Gt (Lit (LInt 0))))]" 
+    using p_before_cfg_to_dag_prog.block_2_def p_before_cfg_to_dag_prog.node_2 by fastforce
+
+  show ?thesis
+    apply (rule generic_ending_block_global_rel)
+          apply (rule syn_rel)
+         apply (rule concrete_trace)
+        apply simp
+       apply simp
+      apply simp
+     apply (rule cmds)
+    apply (rule cfg_is_correct)
+    apply simp
+    done
+qed
+
+
+lemma block_then_global_rel:
+  assumes "A,M,\<Lambda>,\<Gamma>,\<Omega>,T \<turnstile> (bigblock_then, KSeq bigblock1 KStop, (Normal ns1)) -n\<longrightarrow>^j (reached_bb, reached_cont, reached_state)"
+  and  "\<And> m' s'. (red_cfg_multi A M \<Lambda> \<Gamma> \<Omega> p_before_cfg_to_dag_prog.proc_body ((Inl 3),(Normal ns1)) (m',s')) \<Longrightarrow> (s' \<noteq> Failure)"
+  and trace_is_possible: "A,\<Lambda>,\<Gamma>,\<Omega> \<turnstile> \<langle>(BinOp (Var 0) Gt (Lit (LInt 5))), ns1\<rangle> \<Down> LitV (LBool True)"
+  shows "(Ast.valid_configuration A \<Lambda> \<Gamma> \<Omega> [] reached_bb reached_cont reached_state)" 
+proof -
+  have syntactic_rel: "ast_cfg_rel None [] (BigBlock None [(Assign 0 (Lit (LInt 10)))] None None) [(Assign 0 (Lit (LInt 10)))]"
+    by (simp add: Rel_Main_test)
+  have succ: "(out_edges(p_before_cfg_to_dag_prog.proc_body) ! 3) = [2]" 
+    by (simp add: p_before_cfg_to_dag_prog.outEdges_3) 
+
+  show ?thesis 
+    apply (rule block_global_rel_if_true)
+                apply (rule syntactic_rel)
+               apply (rule assms(1))
+              apply simp
+             apply simp
+           apply (rule p_before_cfg_to_dag_prog.node_3)
+          apply (rule p_before_cfg_to_dag_prog.block_3_def)
+          apply (rule assms(2))
+          apply simp
+         apply simp
+        apply simp
+      apply (rule trace_is_possible)
+     apply (rule bigblock_then_local_rel)
+       apply assumption
+      apply assumption
+     apply (rule trace_is_possible)
+    apply (simp add:p_before_cfg_to_dag_prog.outEdges_3)
+    apply ((simp add:member_rec(1)))
+    apply (rule block2_global_rel)
+     apply assumption
+    apply simp
+    done
+qed
+
+
+lemma block_else_global_rel:
+  assumes "A,M,\<Lambda>,\<Gamma>,\<Omega>,T \<turnstile> (bigblock_else, KSeq bigblock1 KStop, (Normal ns1)) -n\<longrightarrow>^j (reached_bb, reached_cont, reached_state)"
+  and  "\<And> m' s'. (red_cfg_multi A M \<Lambda> \<Gamma> \<Omega> p_before_cfg_to_dag_prog.proc_body ((Inl 1),(Normal ns1)) (m',s')) \<Longrightarrow> (s' \<noteq> Failure)"
+  and trace_is_possible: "A,\<Lambda>,\<Gamma>,\<Omega> \<turnstile> \<langle>UnOp Not (BinOp (Var 0) Gt (Lit (LInt 5))), ns1\<rangle> \<Down> LitV (LBool True)"
+  shows "(Ast.valid_configuration A \<Lambda> \<Gamma> \<Omega> [] reached_bb reached_cont reached_state)" 
+proof -
+  have syntactic_rel: "ast_cfg_rel None [] bigblock_else [(Assign 0 (Lit (LInt 1)))]"
+    by (simp add: Rel_Main_test)
+  have succ: "(out_edges (p_before_cfg_to_dag_prog.proc_body) ! Suc 0) = [2]" 
+    using p_before_cfg_to_dag_prog.outEdges_1 by auto 
+  have guard_equiv: "UnOp Not (BinOp (Var 0) Gt (Lit (LInt 5))) \<sim> (Lit (LInt 5) \<guillemotleft>Ge\<guillemotright> Var 0)" 
+    by (rule neg_gt2)
+
+  show ?thesis
+    apply (rule block_global_rel_if_false)
+                apply (rule syntactic_rel)
+               apply (rule assms(1))
+              apply simp
+             apply simp
+            apply (rule p_before_cfg_to_dag_prog.node_1)
+           apply (rule p_before_cfg_to_dag_prog.block_1_def)
+          apply (rule assms(2))
+          apply simp
+         apply simp
+        apply simp
+       apply (rule guard_equiv)
+      apply (rule trace_is_possible)
+     apply (rule bigblock_else_local_rel)
+       apply assumption
+      apply assumption
+     apply (rule trace_is_possible)
+    apply (erule allE[where x=2])
+    apply (simp add: succ)
+    apply (simp add: member_rec(1))
+    apply (rule block2_global_rel)
+     apply assumption
+    apply simp
+    done
+qed
+
+
+lemma block0_global_rel:
+  assumes  "\<And> m' s'. (red_cfg_multi A M \<Lambda> \<Gamma> \<Omega> p_before_cfg_to_dag_prog.proc_body ((Inl 0),(Normal ns1)) (m',s')) \<Longrightarrow> (s' \<noteq> Failure)"
+  and ast_trace: "A,M,\<Lambda>,\<Gamma>,\<Omega>,T \<turnstile> (bigblock0, KSeq bigblock1 KStop, (Normal ns1)) -n\<longrightarrow>^j (reached_bb, reached_cont, reached_state)"
+  shows "(valid_configuration A \<Lambda> \<Gamma> \<Omega> p_before_cfg_to_dag_prog.post reached_bb reached_cont reached_state)" 
+proof -
+  have cmds: "node_to_block(p_before_cfg_to_dag_prog.proc_body) ! 0 = [(Havoc 0)]" 
+    using p_before_cfg_to_dag_prog.block_0_def p_before_cfg_to_dag_prog.node_0 by auto
+  have syntactic_rel: "ast_cfg_rel None [] bigblock0 [Havoc 0]"  
+    by (simp add: Rel_Main_test)
+  have succ: "(out_edges(p_before_cfg_to_dag_prog.proc_body) ! 0) = [3, 1]" 
+    using p_before_cfg_to_dag_prog.outEdges_0 by auto 
+  have "Suc 0 = 1" by simp
+  show ?thesis 
+    apply (rule block_global_rel_if_successor)
+             apply (rule syntactic_rel)
+            apply (rule ast_trace)
+           apply simp
+          apply simp
+        apply (rule cmds)
+       apply (rule assms(1))
+       apply simp
+      apply simp
+     apply (rule bigblock0_local_rel)
+      apply assumption
+     apply assumption
+    apply simp
+    apply (rule disjE)
+      apply assumption
+
+     apply (erule allE[where x=3])
+     apply (simp add:p_before_cfg_to_dag_prog.outEdges_0)
+     apply (simp add:member_rec(1))
+     apply (rule conjE)
+      apply assumption
+    unfolding p_before_cfg_to_dag_prog.post_def
+     apply (rule block_then_global_rel)
+       apply assumption        
+      apply simp
+     apply assumption
+   
+    apply (erule allE[where x=1])
+    apply (simp del: Nat.One_nat_def add:p_before_cfg_to_dag_prog.outEdges_0)
+    apply (simp del: Nat.One_nat_def add:member_rec(1))
+    apply (rule conjE)
+     apply assumption
+    apply (rule block_else_global_rel)
+      apply assumption
+     apply simp
+    apply (simp add: false_equals_not_true)
+    done
+qed
+
+abbreviation \<Lambda>0
+  where
+    "\<Lambda>0  \<equiv> ((append global_data.constants_vdecls global_data.globals_vdecls),(append p_before_cfg_to_dag_prog.params_vdecls p_before_cfg_to_dag_prog.locals_vdecls))"
+lemma end_to_end_theorem_aux3:
+assumes 
+Red: "rtranclp (red_bigblock A M ((append global_data.constants_vdecls global_data.globals_vdecls),(append p_before_cfg_to_dag_prog.params_vdecls p_before_cfg_to_dag_prog.locals_vdecls)) \<Gamma> [] if_example_before_ast_cfg.proc_body) (bigblock0, (KSeq bigblock1 KStop), Normal ns) (end_bb, end_cont, end_state)" and 
+VC: "(\<And> (vc_x::int) (vc_x_0::int) (vc_x_1::int). (vc.vc_anon0 vc_x_0 vc_x_1))" and 
+Closed: "(\<And> v. (closed ((type_of_val A) v)))" and 
+NonEmptyTypes: "(\<And> t. ((closed t) \<Longrightarrow> (\<exists> v. (((type_of_val A) v) = t))))" and 
+FInterp: "(fun_interp_wf A global_data.fdecls \<Gamma>)" and 
+Axioms: "(axiom_assm A \<Gamma> global_data.constants_vdecls (ns::(('a)nstate)) global_data.axioms)" and 
+Precondition: "(expr_all_sat A \<Lambda>0 \<Gamma> [] ns p_before_cfg_to_dag_prog.pres)" and 
+ParamsLocal: "(state_typ_wf A [] (local_state ns) (snd \<Lambda>0))" and 
+ConstsGlobal: "(state_typ_wf A [] (global_state ns) (fst \<Lambda>0))" and 
+OldGlobal: "((global_state ns) = (old_global_state ns))" and 
+BinderNs: "((binder_state ns) = Map.empty)"
+shows "(valid_configuration A \<Lambda>0 \<Gamma> [] p_before_cfg_to_dag_prog.post end_bb end_cont end_state)"
+proof -
+from Red obtain j where Aux:"(A,M,((append global_data.constants_vdecls global_data.globals_vdecls),(append p_before_cfg_to_dag_prog.params_vdecls p_before_cfg_to_dag_prog.locals_vdecls)),\<Gamma>,[],if_example_before_ast_cfg.proc_body \<turnstile> (bigblock0, (KSeq bigblock1 KStop), Normal ns) -n\<longrightarrow>^j (end_bb, end_cont, end_state))"
+by (meson rtranclp_imp_relpowp)
+  show ?thesis
+apply (rule block0_global_rel)
+defer
+apply (rule Aux)
+apply (rule valid_config_implies_not_failure)
+apply (rule end_to_end_theorem_aux)
+apply assumption
+using VC apply simp
+using Closed apply simp
+using NonEmptyTypes apply simp
+apply (rule FInterp)
+using Axioms apply simp
+using Precondition apply simp
+using ParamsLocal apply simp
+using ConstsGlobal apply simp
+using OldGlobal apply simp
+using BinderNs apply simp
+done
+qed
+
+lemma initialization:                              
+  assumes "rtranclp (red_bigblock A M \<Lambda> \<Gamma> \<Omega> T) (init_ast [bigblock0, bigblock1] ns1) (reached_bb, reached_cont, reached_state)"
+  shows "rtranclp (red_bigblock A M \<Lambda> \<Gamma> \<Omega> T) (bigblock0, KSeq bigblock1 KStop, Normal ns1) (reached_bb, reached_cont, reached_state)" 
+proof -
+  have "rtranclp (red_bigblock A M \<Lambda> \<Gamma> \<Omega> T) (bigblock0, convert_list_to_cont (rev [bigblock1]) KStop, Normal ns1) (reached_bb, reached_cont, reached_state)"
+    using assms by fastforce
+  thus ?thesis by simp
+qed
+ 
+
+lemma end_to_end_theorem3:
+assumes 
+VC: "(\<And> (vc_x::int) (vc_x_0::int) (vc_x_1::int). (vc.vc_anon0 vc_x_0 vc_x_1))"
+shows "(\<And> A. (proc_is_correct (A::(('a)absval_ty_fun)) global_data.fdecls global_data.constants_vdecls global_data.globals_vdecls global_data.axioms if_example_before_ast_cfg.proc_ast))"
+  apply (rule end_to_end_util2[OF end_to_end_theorem_aux3])
+apply (rule initialization)
+unfolding if_example_before_ast_cfg.proc_body_def
+apply assumption using VC apply simp  apply assumption+
+       apply (simp_all add: 
+              exprs_to_only_checked_spec_1 exprs_to_only_checked_spec_2
+              if_example_before_ast_cfg.proc_ast_def if_example_before_ast_cfg.proc_body_def 
+              if_example_before_ast_cfg.pres_def if_example_before_ast_cfg.post_def
+              p_before_cfg_to_dag_prog.params_vdecls_def p_before_cfg_to_dag_prog.locals_vdecls_def
+              if_example_before_ast_cfg.params_vdecls_def if_example_before_ast_cfg.locals_vdecls_def
+              p_before_cfg_to_dag_prog.pres_def p_before_cfg_to_dag_prog.post_def)
+       done
+
+end
