BoogieLang/completed_example_proofs/while_example2_proofs/p_proofs/while_example2_ast_cfg_proof.thy
@@ -1,0 +1,535 @@
+theory while_example2_ast_cfg_proof
+  imports Main 
+          Boogie_Lang.Ast
+          Boogie_Lang.Semantics
+          Boogie_Lang.Ast_Cfg_Transformation
+          "../global_data" 
+          p_before_cfg_to_dag_prog 
+          while_example2_before_ast_cfg
+          p_cfgtodag_proof
+          "/home/alex/Isabelle_10-Nov-2021/lib/Apply_Trace_Cmd"
+          p_before_passive_prog 
+          p_passification_proof 
+          p_vcphase_proof
+
+
+(*
+locale ast_to_cfg_lemmas = 
+fixes A :: "(('a)absval_ty_fun)" and \<Gamma> :: "(('a)fun_interp)"
+assumes 
+Wf_Fun: "(fun_interp_wf A global_data.fdecls \<Gamma>)"
+*)
+begin
+
+
+abbreviation \<Lambda>1_local
+  where
+    "\<Lambda>1_local  \<equiv> ((append global_data.constants_vdecls global_data.globals_vdecls),(append p_before_cfg_to_dag_prog.params_vdecls p_before_cfg_to_dag_prog.locals_vdecls))"
+
+abbreviation body_bb1 
+  where "body_bb1 \<equiv> BigBlock None [(Assign 0 (BinOp (Var 0) Sub (Lit (LInt 1))))] None None"
+
+abbreviation body_bb2 
+  where "body_bb2 \<equiv> BigBlock None [(Assign 0 (BinOp (Var 0) Add (Lit (LInt 1))))] None None"
+
+abbreviation unwrapped_bigblock1 where
+  "unwrapped_bigblock1 \<equiv> 
+            (BigBlock None [] 
+            (Some (ParsedWhile (Some (BinOp (Var 0) Lt (Lit (LInt 0)))) 
+                      [(BinOp (Var 0) Le (Lit (LInt 0)))]
+                      [BigBlock None [(Assign 0 (BinOp (Var 0) Add (Lit (LInt 1))))] None None]))
+             None)"
+
+abbreviation loop_only_bigblock0 where
+  "loop_only_bigblock0 \<equiv> 
+            (BigBlock None [] 
+            (Some (WhileWrapper
+                  (ParsedWhile (Some (BinOp (Var 0) Gt (Lit (LInt 0)))) 
+                  [(BinOp (Var 0) Ge (Lit (LInt 0)))]
+                  [BigBlock None [(Assign 0 (BinOp (Var 0) Sub (Lit (LInt 1))))] None None]))) 
+             None)"
+
+abbreviation unwrapped_bigblock0 where
+  "unwrapped_bigblock0 \<equiv> 
+            (BigBlock None [] 
+            (Some (ParsedWhile (Some (BinOp (Var 0) Gt (Lit (LInt 0)))) 
+                      [(BinOp (Var 0) Ge (Lit (LInt 0)))]
+                      [BigBlock None [(Assign 0 (BinOp (Var 0) Sub (Lit (LInt 1))))] None None])) 
+             None)"
+
+lemma bb0_local_rel:
+  assumes Red_bb: "red_bigblock A M \<Lambda>1_local \<Gamma> \<Omega> T (bigblock0, cont0, (Normal ns1)) (reached_bb, reached_cont, reached_state)" 
+  and Red_impl: "(\<And> s2'.((red_cmd_list A M \<Lambda>1_local \<Gamma> \<Omega> p_before_cfg_to_dag_prog.block_0 (Normal ns1) s2') \<Longrightarrow> (s2' \<noteq> Failure)))" 
+  shows "reached_state \<noteq> Failure  \<and>
+         (\<forall>ns1'. reached_state = Normal ns1' \<longrightarrow> (A,M,\<Lambda>1_local,\<Gamma>,\<Omega> \<turnstile> \<langle>p_before_cfg_to_dag_prog.block_0, Normal ns1\<rangle> [\<rightarrow>] Normal ns1'))" 
+proof -
+  have syntactic_rel: "ast_cfg_rel None [] bigblock0 p_before_cfg_to_dag_prog.block_0" 
+    unfolding p_before_cfg_to_dag_prog.block_0_def by (rule Rel_Main_test) 
+  then show ?thesis 
+    using assms
+    unfolding p_before_cfg_to_dag_prog.block_0_def
+    by (auto simp: block_local_rel_generic)
+qed
+
+lemma first_loop_body_bb_local_rel:
+  assumes Red_bb: "red_bigblock A M \<Lambda>1_local \<Gamma> \<Omega> T (body_bb1, cont0, (Normal ns1)) (reached_bb, reached_cont, reached_state)" 
+  and Red_impl: "(\<And> s2'.((red_cmd_list A M \<Lambda>1_local \<Gamma> \<Omega> p_before_cfg_to_dag_prog.block_2 (Normal ns1) s2') \<Longrightarrow> (s2' \<noteq> Failure)))" 
+  and trace_is_possible: "A,\<Lambda>1_local,\<Gamma>,\<Omega> \<turnstile> \<langle>Var 0 \<guillemotleft>Gt\<guillemotright> Lit (LInt 0),ns1\<rangle> \<Down> BoolV True"
+  shows "reached_state \<noteq> Failure  \<and>
+         (\<forall>ns1'. reached_state = Normal ns1' \<longrightarrow> (A,M,\<Lambda>1_local,\<Gamma>,\<Omega> \<turnstile> \<langle>p_before_cfg_to_dag_prog.block_2, Normal ns1\<rangle> [\<rightarrow>] Normal ns1'))" 
+proof -
+  have syntactic_rel: "ast_cfg_rel None [] body_bb1 [(Assign 0 (BinOp (Var 0) Sub (Lit (LInt 1))))]" 
+    by (rule Rel_Main_test) 
+
+  show ?thesis 
+    unfolding p_before_cfg_to_dag_prog.block_2_def
+    apply (rule block_local_rel_guard_true)
+            apply (rule syntactic_rel)
+           apply simp
+          apply simp
+         apply simp
+      apply (rule trace_is_possible)
+     apply (rule Red_bb)
+    apply (rule Red_impl)
+    unfolding p_before_cfg_to_dag_prog.block_2_def
+    by simp
+qed 
+
+lemma second_loop_body_bb_local_rel:
+  assumes Red_bb: "red_bigblock A M \<Lambda>1_local \<Gamma> \<Omega> T (body_bb2, cont0, (Normal ns1)) (reached_bb, reached_cont, reached_state)" 
+  and Red_impl: "(\<And> s2'.((red_cmd_list A M \<Lambda>1_local \<Gamma> \<Omega> p_before_cfg_to_dag_prog.block_5 (Normal ns1) s2') \<Longrightarrow> (s2' \<noteq> Failure)))" 
+  and trace_is_possible: "A,\<Lambda>1_local,\<Gamma>,\<Omega> \<turnstile> \<langle>Var 0 \<guillemotleft>Lt\<guillemotright> Lit (LInt 0),ns1\<rangle> \<Down> BoolV True"
+  shows "reached_state \<noteq> Failure  \<and>
+         (\<forall>ns1'. reached_state = Normal ns1' \<longrightarrow> (A,M,\<Lambda>1_local,\<Gamma>,\<Omega> \<turnstile> \<langle>p_before_cfg_to_dag_prog.block_5, Normal ns1\<rangle> [\<rightarrow>] Normal ns1'))" 
+proof -
+  have syntactic_rel: "ast_cfg_rel None [] body_bb2 [(Assign 0 (BinOp (Var 0) Add (Lit (LInt 1))))]" 
+    by (rule Rel_Main_test) 
+
+  show ?thesis 
+    unfolding p_before_cfg_to_dag_prog.block_5_def
+    apply (rule block_local_rel_guard_true)
+            apply (rule syntactic_rel)
+           apply simp
+          apply simp
+         apply simp
+        apply (rule trace_is_possible)
+      apply (rule Red_bb)
+      apply (rule Red_impl)
+      unfolding p_before_cfg_to_dag_prog.block_5_def
+      by simp
+qed
+
+lemma bb2_local_rel:
+  assumes Red_bb: "red_bigblock A M \<Lambda>1_local \<Gamma> \<Omega> T (bigblock2 , KStop, (Normal ns1)) (reached_bb, reached_cont, reached_state)" 
+  and Red_impl: "(\<And> s2'.((red_cmd_list A M \<Lambda>1_local \<Gamma> \<Omega> p_before_cfg_to_dag_prog.block_6 (Normal ns1) s2') \<Longrightarrow> (s2' \<noteq> Failure)))" 
+  and trace_is_possible: "A,\<Lambda>1_local,\<Gamma>,\<Omega> \<turnstile> \<langle>UnOp Not (BinOp (Var 0) Lt (Lit (LInt 0))), ns1\<rangle> \<Down> BoolV True"
+  shows "reached_state \<noteq> Failure  \<and>
+         (\<forall>ns1'. reached_state = Normal ns1' \<longrightarrow> (A,M,\<Lambda>1_local,\<Gamma>,\<Omega> \<turnstile> \<langle>p_before_cfg_to_dag_prog.block_6, Normal ns1\<rangle> [\<rightarrow>] Normal ns1'))" 
+proof -
+  have syntactic_rel: "ast_cfg_rel None [] bigblock2 [(Assert (BinOp (Var 0) Eq (Lit (LInt 0))))]" 
+    unfolding p_before_cfg_to_dag_prog.block_6_def
+    by (rule Rel_Main_test) 
+  have guard_equiv: "UnOp Not (BinOp (Var 0) Lt (Lit (LInt 0))) \<sim> (Lit (LInt 0) \<guillemotleft>Le\<guillemotright> Var 0)" 
+    by (rule neg_lt2) 
+
+  show ?thesis 
+    unfolding p_before_cfg_to_dag_prog.block_6_def
+    apply (rule block_local_rel_guard_false)
+            apply (rule syntactic_rel)
+           apply simp
+          apply simp
+        apply (rule guard_equiv)
+       apply simp
+      apply (rule trace_is_possible)
+     apply (rule Red_bb)
+    apply (rule Red_impl)
+    unfolding p_before_cfg_to_dag_prog.block_6_def
+    by simp
+qed
+
+lemma bb2_global_rel:
+  assumes concrete_trace: "A,M,\<Lambda>1_local,\<Gamma>,\<Omega>,T \<turnstile> (bigblock2, KStop, (Normal ns1)) -n\<longrightarrow>^j (reached_bb, reached_cont, reached_state)"
+  and cfg_is_correct: "\<And> m' s'. (red_cfg_multi A M \<Lambda>1_local \<Gamma> \<Omega> p_before_cfg_to_dag_prog.proc_body ((Inl 6),(Normal ns1)) (m',s')) \<Longrightarrow> (s' \<noteq> Failure)"
+  and trace_is_possible: "A,\<Lambda>1_local,\<Gamma>,\<Omega> \<turnstile> \<langle>UnOp Not (BinOp (Var 0) Lt (Lit (LInt 0))), ns1\<rangle> \<Down> BoolV True"
+  shows "(Ast.valid_configuration A \<Lambda>1_local \<Gamma> \<Omega> [] reached_bb reached_cont reached_state)" 
+  using assms
+proof -
+  have syn_rel: "ast_cfg_rel None [] bigblock2 [(Assert (BinOp (Var 0) Eq (Lit (LInt 0))))]" by (simp add: Rel_Main_test)
+  have cmds: "node_to_block p_before_cfg_to_dag_prog.proc_body ! 6 = [(Assume (BinOp (Lit (LInt 0)) Le (Var 0))),(Assert (BinOp (Var 0) Eq (Lit (LInt 0))))]" 
+    using p_before_cfg_to_dag_prog.block_6_def p_before_cfg_to_dag_prog.node_6 by auto
+
+  show ?thesis
+    apply (rule generic_ending_block_after_loop_global_rel)
+             apply (rule syn_rel)
+            apply simp
+           apply simp
+          apply simp
+         apply (rule cmds)
+        apply simp
+       apply (rule neg_lt2[of "(Var 0)" "(Lit (LInt 0))"])
+        apply(rule trace_is_possible)
+       apply (rule concrete_trace)
+      apply (rule cfg_is_correct)
+    apply simp
+    done
+qed
+
+
+
+lemma second_loop_body_global_rel:
+  assumes j_step_ast_trace: "A,M,\<Lambda>1_local,\<Gamma>,\<Omega>,T \<turnstile> (body_bb2, (KSeq unwrapped_bigblock1 (KEndBlock (KSeq bigblock2 KStop))), Normal ns1) -n\<longrightarrow>^j (reached_bb, reached_cont, reached_state)"
+  and cfg_is_correct: "\<And> m' s'. (red_cfg_multi A M \<Lambda>1_local \<Gamma> \<Omega> p_before_cfg_to_dag_prog.proc_body ((Inl 5),(Normal ns1)) (m',s')) \<Longrightarrow> (s' \<noteq> Failure)"
+  and trace_is_possible: "A,\<Lambda>1_local,\<Gamma>,\<Omega> \<turnstile> \<langle>Var 0 \<guillemotleft>Lt\<guillemotright> Lit (LInt 0),ns1\<rangle> \<Down> BoolV True"
+  and loop_ih:
+        "\<And>k ns1''. k < j \<Longrightarrow>
+        (A,M,\<Lambda>1_local,\<Gamma>,\<Omega>,T \<turnstile>(unwrapped_bigblock1, (KEndBlock (KSeq bigblock2 KStop)), Normal ns1'') -n\<longrightarrow>^k (reached_bb, reached_cont, reached_state)) \<Longrightarrow>
+        (\<And> m' s'. (red_cfg_multi A M \<Lambda>1_local \<Gamma> \<Omega> p_before_cfg_to_dag_prog.proc_body ((Inl 4),(Normal ns1'')) (m',s')) \<Longrightarrow> (s' \<noteq> Failure)) \<Longrightarrow>
+        (Ast.valid_configuration A \<Lambda>1_local \<Gamma> \<Omega> [] reached_bb reached_cont reached_state)" 
+  shows "(Ast.valid_configuration A \<Lambda>1_local \<Gamma> \<Omega> [] reached_bb reached_cont reached_state)"
+proof -
+  have syn_rel: "ast_cfg_rel None [] body_bb2 [(Assign 0 (BinOp (Var 0) Add (Lit (LInt 1))))]" by (simp add: Rel_Main_test)
+  have cmds: "node_to_block p_before_cfg_to_dag_prog.proc_body ! 5 = [(Assume (BinOp (Var 0) Lt (Lit (LInt 0)))),(Assign 0 (BinOp (Var 0) Add (Lit (LInt 1))))]" 
+    using p_before_cfg_to_dag_prog.block_5_def p_before_cfg_to_dag_prog.node_5 by fastforce
+  show ?thesis
+    apply (rule block_global_rel_if_true)
+               apply (rule syn_rel)
+              apply (rule j_step_ast_trace)
+             apply simp
+            apply simp
+           apply (rule cmds)
+          apply simp
+         apply (rule cfg_is_correct)
+         apply simp
+        apply simp
+       apply simp
+      apply (rule trace_is_possible)
+     apply (rule block_local_rel_guard_true)
+           apply (rule syn_rel)
+          apply (simp, simp, simp)
+       apply (rule trace_is_possible)
+      apply assumption
+     apply assumption
+    apply (simp add: p_before_cfg_to_dag_prog.outEdges_5)
+    apply (simp add: member_rec)
+    apply (rule loop_ih)
+      apply auto
+    done
+qed
+
+lemma second_loop_head_global_rel:
+  assumes j_step_ast_trace: "A,M,\<Lambda>1_local,\<Gamma>,\<Omega>,T \<turnstile> (unwrapped_bigblock1, (KEndBlock (KSeq bigblock2 KStop)), Normal ns1) -n\<longrightarrow>^j (reached_bb, reached_cont, reached_state)"
+  and cfg_is_correct: "\<And> m' s'. (red_cfg_multi A M \<Lambda>1_local \<Gamma> \<Omega> p_before_cfg_to_dag_prog.proc_body ((Inl 4),(Normal ns1)) (m',s')) \<Longrightarrow> (s' \<noteq> Failure)"
+  shows "(Ast.valid_configuration A \<Lambda>1_local \<Gamma> \<Omega> [] reached_bb reached_cont reached_state)"
+  using assms
+proof (induction j arbitrary: ns1 rule: less_induct)
+  case (less j)
+  then show ?case 
+  proof (cases j)
+    case 0
+    then show ?thesis
+      using Ast.valid_configuration_def less.prems(1) by fastforce
+  next
+    case (Suc j')
+    have ast_cfg_rel_concrete sorry
+
+    have transfer_all: "(\<forall>m3 s3 n ns. ((A,M,\<Lambda>1_local,\<Gamma>,\<Omega>,G \<turnstile>(Inl n, Normal ns) -n\<rightarrow>* (m3, s3)) \<longrightarrow> s3 \<noteq> Failure)) \<Longrightarrow> 
+                        (\<And>m3 s3 n ns. ((A,M,\<Lambda>1_local,\<Gamma>,\<Omega>,G \<turnstile>(Inl n, Normal ns) -n\<rightarrow>* (m3, s3)) \<Longrightarrow> s3 \<noteq> Failure))" by auto
+
+    have node_4_helper: "node_to_block p_before_cfg_to_dag_prog.proc_body ! 4 = [Assert (Var 0 \<guillemotleft>Le\<guillemotright> Lit (LInt 0))]" 
+      by (simp add: p_before_cfg_to_dag_prog.block_4_def p_before_cfg_to_dag_prog.node_4)
+    show ?thesis
+      apply (rule block_global_rel_loop_head)
+             apply (rule Rel_Invs)
+            apply (rule less(2))
+           apply (rule less(3))
+           apply simp
+          apply simp                 
+         apply (rule block_local_rel_loop_head)
+            apply (rule Rel_Invs)
+           apply simp
+          apply simp
+         apply simp
+        apply simp
+       apply simp
+       apply (rule node_4_helper)
+      apply(rule disjE)
+        apply assumption
+
+       apply (erule allE[where x = 5])
+       apply (simp add:p_before_cfg_to_dag_prog.outEdges_4)
+       apply (simp add:member_rec(1))
+       apply (rule conjE)
+        apply assumption
+       apply simp
+       apply (rule second_loop_body_global_rel)
+          apply assumption
+         apply simp
+        apply assumption
+       apply (rule less.IH)
+         apply (erule strictly_smaller_helper2)
+         apply assumption
+         apply assumption
+       apply assumption
+
+      apply (erule allE[where x = 6])
+      apply (simp add:p_before_cfg_to_dag_prog.outEdges_4)
+      apply (simp add:member_rec(1))
+      apply (rule conjE)
+       apply assumption
+      apply simp
+      apply (rule ending)
+          apply assumption
+         apply assumption 
+        (* using allE impCE notE HOL.refl subst sym swap arity_type_nat impI notI rev_mp RedVar_case RedBinOp_case arity_type_state arity_type_val *)
+        apply blast
+        apply assumption
+       apply (simp add: bb2_global_rel)
+   (* TODO: Here auto works after deferring, otherwise it doesn't, why? 
+      Answer: it works without deferring as well but then it changes the other subgoals also. 'subgoal by auto' doesn't work. Why? *)
+   (* apply_trace auto *)
+      done
+  qed
+qed
+
+lemma first_loop_body_global_rel:
+  assumes j_step_ast_trace: 
+    "A,M,\<Lambda>1_local,\<Gamma>,\<Omega>,T \<turnstile> (body_bb1, (KSeq unwrapped_bigblock0 (KEndBlock (KSeq bigblock1 (KSeq bigblock2 KStop)))), Normal ns1) -n\<longrightarrow>^j (reached_bb, reached_cont, reached_state)"
+  and cfg_is_correct: "\<And> m' s'. (red_cfg_multi A M \<Lambda>1_local \<Gamma> \<Omega> p_before_cfg_to_dag_prog.proc_body ((Inl 2),(Normal ns1)) (m',s')) \<Longrightarrow> (s' \<noteq> Failure)"
+  and trace_is_possible: "A,\<Lambda>1_local,\<Gamma>,\<Omega> \<turnstile> \<langle>Var 0 \<guillemotleft>Gt\<guillemotright> Lit (LInt 0), ns1\<rangle> \<Down> BoolV True"
+  and loop_ih:
+        "\<And>k ns1''. k < j \<Longrightarrow>
+        (A,M,\<Lambda>1_local,\<Gamma>,\<Omega>,T \<turnstile>(unwrapped_bigblock0, (KEndBlock (KSeq bigblock1 (KSeq bigblock2 KStop))), Normal ns1'') -n\<longrightarrow>^k (reached_bb, reached_cont, reached_state)) \<Longrightarrow>
+        (\<And> m' s'. (red_cfg_multi A M \<Lambda>1_local \<Gamma> \<Omega> p_before_cfg_to_dag_prog.proc_body ((Inl 1),(Normal ns1'')) (m',s')) \<Longrightarrow> (s' \<noteq> Failure)) \<Longrightarrow>
+        (Ast.valid_configuration A \<Lambda>1_local \<Gamma> \<Omega> [] reached_bb reached_cont reached_state)"  shows "(Ast.valid_configuration A \<Lambda>1_local \<Gamma> \<Omega> [] reached_bb reached_cont reached_state)"
+proof -
+  have syn_rel: "ast_cfg_rel None [] body_bb1 [(Assign 0 (BinOp (Var 0) Sub (Lit (LInt 1))))]" by (simp add: Rel_Main_test)
+  have cmds: "node_to_block p_before_cfg_to_dag_prog.proc_body ! 2 = [(Assume (BinOp (Var 0) Gt (Lit (LInt 0)))),(Assign 0 (BinOp (Var 0) Sub (Lit (LInt 1))))]" 
+    using p_before_cfg_to_dag_prog.block_2_def p_before_cfg_to_dag_prog.node_2 by fastforce
+  show ?thesis
+    apply (rule block_global_rel_if_true)
+               apply (rule syn_rel)
+              apply (rule j_step_ast_trace)
+             apply simp
+            apply simp
+           apply (rule cmds)
+          apply simp
+         apply (rule cfg_is_correct)
+         apply simp
+        apply simp
+       apply simp
+      apply (rule trace_is_possible)
+     apply (rule block_local_rel_guard_true)
+           apply (rule syn_rel)
+          apply (simp, simp, simp)
+       apply (rule trace_is_possible)
+      apply assumption
+     apply assumption
+    apply (simp add: p_before_cfg_to_dag_prog.outEdges_2)
+    apply (simp add: member_rec)
+    apply (rule loop_ih)
+      apply auto
+    done
+qed
+
+
+lemma correctness_propagates_through_assumption_concrete:
+  assumes "\<forall>m s. (A,M,\<Lambda>1_local,\<Gamma>,\<Omega>,p_before_cfg_to_dag_prog.proc_body \<turnstile> (Inl 3, Normal ns1) -n\<rightarrow>* (m, s)) \<longrightarrow> s \<noteq> Failure"
+      and "node_to_block p_before_cfg_to_dag_prog.proc_body ! 3 = [Assume c]"
+      and "UnOp Not guard \<sim> c"
+      and "A,\<Lambda>1_local,\<Gamma>,\<Omega> \<turnstile> \<langle>guard, ns1\<rangle> \<Down> BoolV False"
+    shows "\<And>m1 s1. (A,M,\<Lambda>1_local,\<Gamma>,\<Omega>,p_before_cfg_to_dag_prog.proc_body \<turnstile> (Inl 4, Normal ns1) -n\<rightarrow>* (m1, s1)) \<Longrightarrow> s1 \<noteq> Failure"
+  using assms
+proof -
+  have succ: "List.member [4] 4" by (simp add: member_rec(1))
+  fix m1 s1
+  assume prem: "(A,M,\<Lambda>1_local,\<Gamma>,\<Omega>,p_before_cfg_to_dag_prog.proc_body \<turnstile> (Inl 4, Normal ns1) -n\<rightarrow>* (m1, s1))"
+  show "s1 \<noteq> Failure"
+  apply (rule correctness_propagates_through_assumption)
+       apply (rule assms(1))
+      apply (rule assms(2))
+     apply (rule assms(3))
+    apply (rule assms(4))
+     apply (simp add: p_before_cfg_to_dag_prog.outEdges_3)
+     apply (rule succ)
+    apply (rule prem)
+    done
+qed
+
+lemma first_loop_head_global_rel:
+  assumes j_step_ast_trace: 
+    "A,M,\<Lambda>1_local,\<Gamma>,\<Omega>,T \<turnstile> (unwrapped_bigblock0, (KEndBlock (KSeq bigblock1 (KSeq bigblock2 KStop))), Normal ns1) -n\<longrightarrow>^j (reached_bb, reached_cont, reached_state)"
+  and cfg_is_correct: "\<And> m' s'. (red_cfg_multi A M \<Lambda>1_local \<Gamma> \<Omega> p_before_cfg_to_dag_prog.proc_body ((Inl 1),(Normal ns1)) (m',s')) \<Longrightarrow> (s' \<noteq> Failure)"
+  shows "(Ast.valid_configuration A \<Lambda>1_local \<Gamma> \<Omega> [] reached_bb reached_cont reached_state)"
+  using assms 
+proof (induction j arbitrary: ns1 rule: less_induct)
+  case (less j)
+  then show ?case 
+  proof (cases j)
+    case 0
+    then show ?thesis
+      using valid_configuration_def less.prems(1) by fastforce
+  next
+    case (Suc j')
+    have out_edges_Suc0: "((nth (out_edges p_before_cfg_to_dag_prog.proc_body) (Suc 0)) = [3,2])" using p_before_cfg_to_dag_prog.outEdges_1 by auto
+    have node_3_helper: "node_to_block p_before_cfg_to_dag_prog.proc_body ! 3 = [(Assume (BinOp (Lit (LInt 0)) Ge (Var 0)))]" 
+      using p_before_cfg_to_dag_prog.block_3_def p_before_cfg_to_dag_prog.node_3 by auto
+    have node_1_helper: "node_to_block p_before_cfg_to_dag_prog.proc_body ! (Suc 0) = [Assert (Var 0 \<guillemotleft>Ge\<guillemotright> Lit (LInt 0))]" 
+      using p_before_cfg_to_dag_prog.block_1_def p_before_cfg_to_dag_prog.node_1 by auto
+    have succ_helper: "List.member [4] 4"by (simp add: member_rec(1))
+    show ?thesis
+      apply (rule block_global_rel_loop_head) 
+             apply (rule Rel_Invs)
+            apply (rule less(2))
+           apply (rule less(3))
+           apply simp
+          apply simp                 
+         apply (rule block_local_rel_loop_head)
+            apply (rule Rel_Invs)
+           apply simp
+          apply simp
+         apply simp
+        apply simp
+       apply simp
+       apply (rule node_1_helper)
+      apply(rule disjE)
+        apply assumption
+    
+       apply (erule allE[where x = 2])
+       apply (simp add: out_edges_Suc0)
+       apply (simp add:member_rec(1))
+       apply (rule conjE)
+        apply assumption
+       apply simp
+       apply (rule first_loop_body_global_rel)
+          apply assumption
+         apply simp
+        apply assumption
+       apply (rule less.IH)
+         apply (erule strictly_smaller_helper2)
+         apply assumption
+         apply assumption
+       apply assumption
+
+      apply (erule allE[where x = 3])
+      apply (simp add:out_edges_Suc0)
+      apply (simp add:member_rec(1))
+      apply (rule conjE)
+       apply assumption
+      apply simp
+      apply (rule ending2)
+             apply assumption
+            apply assumption
+           apply assumption
+          apply assumption
+         apply (rule node_3_helper)
+        apply (rule neg_gt2)
+       apply (simp add: p_before_cfg_to_dag_prog.outEdges_3)
+       apply (rule succ_helper)
+      by (simp add: second_loop_head_global_rel)
+  qed
+qed
+
+lemma entry_block_global_rel:
+  assumes j_step_ast_trace: 
+    "A,M,\<Lambda>1_local,\<Gamma>,\<Omega>,T \<turnstile> (bigblock0, (KSeq bigblock1 (KSeq bigblock2 KStop)), Normal ns1) -n\<longrightarrow>^j (reached_bb, reached_cont, reached_state)"
+  and cfg_is_correct: "\<And> m' s'. (red_cfg_multi A M \<Lambda>1_local \<Gamma> \<Omega> p_before_cfg_to_dag_prog.proc_body ((Inl 0),(Normal ns1)) (m',s')) \<Longrightarrow> (s' \<noteq> Failure)"
+  shows "(Ast.valid_configuration A \<Lambda>1_local \<Gamma> \<Omega> p_before_cfg_to_dag_prog.post reached_bb reached_cont reached_state)"
+  using assms
+proof -
+  have node_0_helper: "node_to_block p_before_cfg_to_dag_prog.proc_body ! 0 = [Havoc 0]" 
+    by (simp add: p_before_cfg_to_dag_prog.block_0_def p_before_cfg_to_dag_prog.node_0)
+  have "[Havoc 0] = p_before_cfg_to_dag_prog.block_0" by (simp only: p_before_cfg_to_dag_prog.block_0_def) 
+  show ?thesis
+    unfolding p_before_cfg_to_dag_prog.post_def
+    apply (rule block_global_rel_while_successor)
+          apply (rule j_step_ast_trace)
+         apply (rule Rel_Main_test)
+        apply simp
+       apply (rule node_0_helper)
+      apply (rule cfg_is_correct)
+      apply simp
+     apply (simp only: \<open>[Havoc 0] = p_before_cfg_to_dag_prog.block_0\<close>)
+     apply (rule bb0_local_rel)
+      apply (simp only: \<open>[Havoc 0] = p_before_cfg_to_dag_prog.block_0\<close>)
+     apply assumption
+    apply (simp del: Nat.One_nat_def add: p_before_cfg_to_dag_prog.outEdges_0)
+    apply (simp del: Nat.One_nat_def add: member_rec)
+    apply (rule first_loop_head_global_rel)
+     apply assumption
+    (* TODO: Again, why does auto work only in the end here? *)
+    by auto
+qed
+
+abbreviation \<Lambda>0_local
+  where
+    "\<Lambda>0_local  \<equiv> ((append global_data.constants_vdecls global_data.globals_vdecls),(append p_before_cfg_to_dag_prog.params_vdecls p_before_cfg_to_dag_prog.locals_vdecls))"
+lemma end_to_end_theorem_aux2:
+assumes 
+Red: "rtranclp (red_bigblock 
+      A M ((append global_data.constants_vdecls global_data.globals_vdecls),(append p_before_cfg_to_dag_prog.params_vdecls p_before_cfg_to_dag_prog.locals_vdecls)) \<Gamma> [] 
+            while_example2_before_ast_cfg.proc_body) 
+      (bigblock0, (KSeq bigblock1 (KSeq bigblock2 KStop)), Normal ns) (end_bb, end_cont, end_state)" and 
+VC: "(\<And> (vc_x::int) (vc_x_0::int) (vc_x_1::int) (vc_x_2::int) (vc_x_3::int) (vc_x_4::int). (vc.vc_PreconditionGeneratedEntry vc_x_0 vc_x_1 vc_x_3 vc_x_4 vc_x_2))" and 
+Closed: "(\<And> v. (closed ((type_of_val A) v)))" and 
+NonEmptyTypes: "(\<And> t. ((closed t) \<Longrightarrow> (\<exists> v. (((type_of_val A) v) = t))))" and 
+FInterp: "(fun_interp_wf A global_data.fdecls \<Gamma>)" and 
+Axioms: "(axiom_assm A \<Gamma> global_data.constants_vdecls (ns::(('a)nstate)) global_data.axioms)" and 
+Precondition: "(expr_all_sat A \<Lambda>0_local \<Gamma> [] ns p_before_cfg_to_dag_prog.pres)" and 
+ParamsLocal: "(state_typ_wf A [] (local_state ns) (snd \<Lambda>0_local))" and 
+ConstsGlobal: "(state_typ_wf A [] (global_state ns) (fst \<Lambda>0_local))" and 
+OldGlobal: "((global_state ns) = (old_global_state ns))" and 
+BinderNs: "((binder_state ns) = Map.empty)"
+shows "(Ast.valid_configuration A \<Lambda>0_local \<Gamma> [] p_before_cfg_to_dag_prog.post end_bb end_cont end_state)"
+proof -
+  from Red obtain j where 
+    Aux:"(A,M,((append global_data.constants_vdecls global_data.globals_vdecls),(append p_before_cfg_to_dag_prog.params_vdecls p_before_cfg_to_dag_prog.locals_vdecls)),\<Gamma>,[],while_example2_before_ast_cfg.proc_body \<turnstile> (bigblock0, (KSeq bigblock1 (KSeq bigblock2 KStop)), Normal ns) -n\<longrightarrow>^j (end_bb, end_cont, end_state))"
+by (meson rtranclp_imp_relpowp)
+  show ?thesis
+apply (rule entry_block_global_rel)
+apply (rule Aux)
+apply (rule valid_config_implies_not_failure)
+apply (rule end_to_end_theorem_aux)
+apply assumption
+using VC apply simp
+using Closed apply simp
+using NonEmptyTypes apply simp
+apply (rule FInterp)
+using Axioms apply simp
+using Precondition apply simp
+using ParamsLocal apply simp
+using ConstsGlobal apply simp
+using OldGlobal apply simp
+using BinderNs apply simp
+done
+qed
+
+lemma initialization:                              
+  assumes "rtranclp (red_bigblock A M \<Lambda> \<Gamma> \<Omega> T) (init_ast [bigblock0, bigblock1, bigblock2] ns1) (reached_bb, reached_cont, reached_state)"
+  shows "rtranclp (red_bigblock A M \<Lambda> \<Gamma> \<Omega> T) (bigblock0, KSeq bigblock1 (KSeq bigblock2 KStop), Normal ns1) (reached_bb, reached_cont, reached_state)" 
+proof -
+  have "rtranclp (red_bigblock A M \<Lambda> \<Gamma> \<Omega> T) (bigblock0, convert_list_to_cont (rev [bigblock1, bigblock2]) KStop, Normal ns1) (reached_bb, reached_cont, reached_state)"
+    using assms by fastforce
+  hence "rtranclp (red_bigblock A M \<Lambda> \<Gamma> \<Omega> T) (bigblock0, convert_list_to_cont (rev [bigblock1]) (KSeq bigblock2 KStop), Normal ns1) (reached_bb, reached_cont, reached_state)"
+    by simp
+  thus ?thesis by simp
+qed
+ 
+
+lemma end_to_end_theorem2:
+assumes 
+VC: "(\<And> (vc_x::int) (vc_x_0::int) (vc_x_1::int) (vc_x_2::int) (vc_x_3::int) (vc_x_4::int). (vc.vc_PreconditionGeneratedEntry vc_x_0 vc_x_1 vc_x_3 vc_x_4 vc_x_2))"
+shows "(\<And> A. (Ast.proc_is_correct (A::(('a)absval_ty_fun)) global_data.fdecls global_data.constants_vdecls global_data.globals_vdecls global_data.axioms while_example2_before_ast_cfg.proc_ast))"
+apply (rule end_to_end_util2[OF end_to_end_theorem_aux2])
+apply (rule initialization)
+unfolding while_example2_before_ast_cfg.proc_body_def
+apply assumption using VC apply simp  apply assumption+
+  unfolding p_before_cfg_to_dag_prog.pres_def p_before_cfg_to_dag_prog.post_def
+       apply (simp_all add: 
+              exprs_to_only_checked_spec_1 exprs_to_only_checked_spec_2
+              while_example2_before_ast_cfg.proc_ast_def while_example2_before_ast_cfg.proc_body_def 
+              while_example2_before_ast_cfg.pres_def while_example2_before_ast_cfg.post_def
+              p_before_cfg_to_dag_prog.params_vdecls_def p_before_cfg_to_dag_prog.locals_vdecls_def
+              while_example2_before_ast_cfg.params_vdecls_def while_example2_before_ast_cfg.locals_vdecls_def)
+  done
+
+end
